QCP_examples/humaneval/spec_logic_rewrite_c_files/C_103_goal.v
@@ -1,0 +1,1430 @@
+Require Import Coq.ZArith.ZArith.
+Require Import Coq.Bool.Bool.
+Require Import Coq.Strings.String.
+Require Import Coq.Strings.Ascii.
+Require Import Coq.Lists.List.
+Require Import Coq.Classes.RelationClasses.
+Require Import Coq.Classes.Morphisms.
+Require Import Coq.micromega.Psatz.
+Require Import Coq.Sorting.Permutation.
+From AUXLib Require Import int_auto Axioms Feq Idents ListLib VMap.
+Require Import SetsClass.SetsClass. Import SetsNotation.
+From SimpleC.SL Require Import Mem SeparationLogic.
+Require Import Logic.LogicGenerator.demo932.Interface.
+Local Open Scope Z_scope.
+Local Open Scope sets.
+Local Open Scope string_scope.
+Local Open Scope list.
+Import naive_C_Rules.
+Require Import SimpleC.StdLib.string_lib.
+Require Import coins_103.
+Local Open Scope sac.
+From SimpleC.EE.QCP_demos_LLM Require Import char_array_strategy_goal.
+From SimpleC.EE.QCP_demos_LLM Require Import char_array_strategy_proof.
+From SimpleC.StdLib Require Import string_strategy_goal.
+From SimpleC.StdLib Require Import string_strategy_proof.
+
+(*----- Function to_binary_string -----*)
+
+Definition to_binary_string_safety_wit_1 := 
+forall (num_pre: Z) (PreH1 : (0 <= num_pre)) (PreH2 : (num_pre <= INT_MAX)) (PreH3 : (binary_safe_103 num_pre )) ,
+  ((( &( "bits" ) )) # Int  |->_)
+  **  ((( &( "num" ) )) # Int  |-> num_pre)
+|--
+  “ (0 <= INT_MAX) ” 
+  &&  “ ((INT_MIN) <= 0) ”
+.
+
+Definition to_binary_string_safety_wit_2 := 
+forall (num_pre: Z) (PreH1 : (0 <= num_pre)) (PreH2 : (num_pre <= INT_MAX)) (PreH3 : (binary_safe_103 num_pre )) ,
+  ((( &( "out" ) )) # Ptr  |->_)
+  **  ((( &( "x" ) )) # Int  |-> num_pre)
+  **  ((( &( "bits" ) )) # Int  |-> 0)
+  **  ((( &( "num" ) )) # Int  |-> num_pre)
+|--
+  “ (0 <= INT_MAX) ” 
+  &&  “ ((INT_MIN) <= 0) ”
+.
+
+Definition to_binary_string_safety_wit_3 := 
+forall (num_pre: Z) (PreH1 : (0 <= num_pre)) (PreH2 : (num_pre <= INT_MAX)) (PreH3 : (binary_safe_103 num_pre )) ,
+  ((( &( "out" ) )) # Ptr  |-> 0)
+  **  ((( &( "x" ) )) # Int  |-> num_pre)
+  **  ((( &( "bits" ) )) # Int  |-> 0)
+  **  ((( &( "num" ) )) # Int  |-> num_pre)
+|--
+  “ (0 <= INT_MAX) ” 
+  &&  “ ((INT_MIN) <= 0) ”
+.
+
+Definition to_binary_string_safety_wit_4 := 
+forall (num_pre: Z) (PreH1 : (num_pre = 0)) (PreH2 : (0 <= num_pre)) (PreH3 : (num_pre <= INT_MAX)) (PreH4 : (binary_safe_103 num_pre )) ,
+  ((( &( "out" ) )) # Ptr  |-> 0)
+  **  ((( &( "x" ) )) # Int  |-> num_pre)
+  **  ((( &( "bits" ) )) # Int  |-> 0)
+  **  ((( &( "num" ) )) # Int  |-> num_pre)
+|--
+  “ (2 <= INT_MAX) ” 
+  &&  “ ((INT_MIN) <= 2) ”
+.
+
+Definition to_binary_string_safety_wit_5 := 
+forall (num_pre: Z) (retval: Z) (PreH1 : (retval <> 0)) (PreH2 : (num_pre = 0)) (PreH3 : (0 <= num_pre)) (PreH4 : (num_pre <= INT_MAX)) (PreH5 : (binary_safe_103 num_pre )) ,
+  (CharArray.undef_full retval 2 )
+  **  ((( &( "out" ) )) # Ptr  |-> retval)
+  **  ((( &( "x" ) )) # Int  |-> num_pre)
+  **  ((( &( "bits" ) )) # Int  |-> 0)
+  **  ((( &( "num" ) )) # Int  |-> num_pre)
+|--
+  “ (0 <= INT_MAX) ” 
+  &&  “ ((INT_MIN) <= 0) ”
+.
+
+Definition to_binary_string_safety_wit_6 := 
+forall (num_pre: Z) (retval: Z) (PreH1 : (retval <> 0)) (PreH2 : (num_pre = 0)) (PreH3 : (0 <= num_pre)) (PreH4 : (num_pre <= INT_MAX)) (PreH5 : (binary_safe_103 num_pre )) ,
+  (CharArray.undef_full retval 2 )
+  **  ((( &( "out" ) )) # Ptr  |-> retval)
+  **  ((( &( "x" ) )) # Int  |-> num_pre)
+  **  ((( &( "bits" ) )) # Int  |-> 0)
+  **  ((( &( "num" ) )) # Int  |-> num_pre)
+|--
+  “ (48 <= INT_MAX) ” 
+  &&  “ ((INT_MIN) <= 48) ”
+.
+
+Definition to_binary_string_safety_wit_7 := 
+forall (num_pre: Z) (retval: Z) (PreH1 : (retval <> 0)) (PreH2 : (num_pre = 0)) (PreH3 : (0 <= num_pre)) (PreH4 : (num_pre <= INT_MAX)) (PreH5 : (binary_safe_103 num_pre )) ,
+  (CharArray.undef_seg retval (0 + 1 ) 2 )
+  **  (((retval + (0 * sizeof(CHAR) ) )) # Char  |-> 48)
+  **  ((( &( "out" ) )) # Ptr  |-> retval)
+  **  ((( &( "x" ) )) # Int  |-> num_pre)
+  **  ((( &( "bits" ) )) # Int  |-> 0)
+  **  ((( &( "num" ) )) # Int  |-> num_pre)
+|--
+  “ (1 <= INT_MAX) ” 
+  &&  “ ((INT_MIN) <= 1) ”
+.
+
+Definition to_binary_string_safety_wit_8 := 
+forall (num_pre: Z) (retval: Z) (PreH1 : (retval <> 0)) (PreH2 : (num_pre = 0)) (PreH3 : (0 <= num_pre)) (PreH4 : (num_pre <= INT_MAX)) (PreH5 : (binary_safe_103 num_pre )) ,
+  (CharArray.undef_seg retval (0 + 1 ) 2 )
+  **  (((retval + (0 * sizeof(CHAR) ) )) # Char  |-> 48)
+  **  ((( &( "out" ) )) # Ptr  |-> retval)
+  **  ((( &( "x" ) )) # Int  |-> num_pre)
+  **  ((( &( "bits" ) )) # Int  |-> 0)
+  **  ((( &( "num" ) )) # Int  |-> num_pre)
+|--
+  “ (0 <= INT_MAX) ” 
+  &&  “ ((INT_MIN) <= 0) ”
+.
+
+Definition to_binary_string_safety_wit_9 := 
+forall (num_pre: Z) (out: Z) (bits: Z) (x: Z) (PreH1 : (0 < num_pre)) (PreH2 : (num_pre <= INT_MAX)) (PreH3 : (0 <= x)) (PreH4 : (0 <= bits)) (PreH5 : (out = 0)) (PreH6 : (binary_safe_103 num_pre )) (PreH7 : (binary_count_state_z_103 num_pre x bits )) ,
+  ((( &( "num" ) )) # Int  |-> num_pre)
+  **  ((( &( "x" ) )) # Int  |-> x)
+  **  ((( &( "bits" ) )) # Int  |-> bits)
+  **  ((( &( "out" ) )) # Ptr  |-> out)
+|--
+  “ (0 <= INT_MAX) ” 
+  &&  “ ((INT_MIN) <= 0) ”
+.
+
+Definition to_binary_string_safety_wit_10 := 
+(
+forall (num_pre: Z) (out: Z) (bits: Z) (x: Z) (PreH1 : (x > 0)) (PreH2 : (0 < num_pre)) (PreH3 : (num_pre <= INT_MAX)) (PreH4 : (0 <= x)) (PreH5 : (0 <= bits)) (PreH6 : (out = 0)) (PreH7 : (binary_safe_103 num_pre )) (PreH8 : (binary_count_state_z_103 num_pre x bits )) ,
+  ((( &( "num" ) )) # Int  |-> num_pre)
+  **  ((( &( "x" ) )) # Int  |-> x)
+  **  ((( &( "bits" ) )) # Int  |-> bits)
+  **  ((( &( "out" ) )) # Ptr  |-> out)
+|--
+  “ ((bits + 1 ) <= INT_MAX) ” 
+  &&  “ ((INT_MIN) <= (bits + 1 )) ”
+) \/
+(
+forall (num_pre: Z) (out: Z) (bits: Z) (x: Z) (PreH1 : (x > 0)) (PreH2 : (0 < num_pre)) (PreH3 : (num_pre <= INT_MAX)) (PreH4 : (0 <= x)) (PreH5 : (0 <= bits)) (PreH6 : (out = 0)) (PreH7 : (binary_safe_103 num_pre )) (PreH8 : (binary_count_state_z_103 num_pre x bits )) ,
+  ((( &( "num" ) )) # Int  |-> num_pre)
+  **  ((( &( "x" ) )) # Int  |-> x)
+  **  ((( &( "bits" ) )) # Int  |-> bits)
+  **  ((( &( "out" ) )) # Ptr  |-> out)
+|--
+  “ ((bits + 1 ) <= INT_MAX) ” 
+  &&  “ ((INT_MIN) <= (bits + 1 )) ”
+).
+
+Definition to_binary_string_safety_wit_10_split_goal_1 := 
+forall (num_pre: Z) (out: Z) (bits: Z) (x: Z) (PreH1 : (x > 0)) (PreH2 : (0 < num_pre)) (PreH3 : (num_pre <= INT_MAX)) (PreH4 : (0 <= x)) (PreH5 : (0 <= bits)) (PreH6 : (out = 0)) (PreH7 : (binary_safe_103 num_pre )) (PreH8 : (binary_count_state_z_103 num_pre x bits )) ,
+  ((( &( "num" ) )) # Int  |-> num_pre)
+  **  ((( &( "x" ) )) # Int  |-> x)
+  **  ((( &( "bits" ) )) # Int  |-> bits)
+  **  ((( &( "out" ) )) # Ptr  |-> out)
+|--
+  “ ((bits + 1 ) <= INT_MAX) ”
+.
+
+Definition to_binary_string_safety_wit_10_split_goal_2 := 
+forall (num_pre: Z) (out: Z) (bits: Z) (x: Z) (PreH1 : (x > 0)) (PreH2 : (0 < num_pre)) (PreH3 : (num_pre <= INT_MAX)) (PreH4 : (0 <= x)) (PreH5 : (0 <= bits)) (PreH6 : (out = 0)) (PreH7 : (binary_safe_103 num_pre )) (PreH8 : (binary_count_state_z_103 num_pre x bits )) ,
+  ((( &( "num" ) )) # Int  |-> num_pre)
+  **  ((( &( "x" ) )) # Int  |-> x)
+  **  ((( &( "bits" ) )) # Int  |-> bits)
+  **  ((( &( "out" ) )) # Ptr  |-> out)
+|--
+  “ ((INT_MIN) <= (bits + 1 )) ”
+.
+
+Definition to_binary_string_safety_wit_11 := 
+forall (num_pre: Z) (out: Z) (bits: Z) (x: Z) (PreH1 : (x > 0)) (PreH2 : (0 < num_pre)) (PreH3 : (num_pre <= INT_MAX)) (PreH4 : (0 <= x)) (PreH5 : (0 <= bits)) (PreH6 : (out = 0)) (PreH7 : (binary_safe_103 num_pre )) (PreH8 : (binary_count_state_z_103 num_pre x bits )) ,
+  ((( &( "num" ) )) # Int  |-> num_pre)
+  **  ((( &( "x" ) )) # Int  |-> x)
+  **  ((( &( "bits" ) )) # Int  |-> bits)
+  **  ((( &( "out" ) )) # Ptr  |-> out)
+|--
+  “ (1 <= INT_MAX) ” 
+  &&  “ ((INT_MIN) <= 1) ”
+.
+
+Definition to_binary_string_safety_wit_12 := 
+forall (num_pre: Z) (out: Z) (bits: Z) (x: Z) (PreH1 : (x > 0)) (PreH2 : (0 < num_pre)) (PreH3 : (num_pre <= INT_MAX)) (PreH4 : (0 <= x)) (PreH5 : (0 <= bits)) (PreH6 : (out = 0)) (PreH7 : (binary_safe_103 num_pre )) (PreH8 : (binary_count_state_z_103 num_pre x bits )) ,
+  ((( &( "num" ) )) # Int  |-> num_pre)
+  **  ((( &( "x" ) )) # Int  |-> x)
+  **  ((( &( "bits" ) )) # Int  |-> (bits + 1 ))
+  **  ((( &( "out" ) )) # Ptr  |-> out)
+|--
+  “ ((x <> (INT_MIN)) \/ (2 <> (-1))) ” 
+  &&  “ (2 <> 0) ”
+.
+
+Definition to_binary_string_safety_wit_13 := 
+forall (num_pre: Z) (out: Z) (bits: Z) (x: Z) (PreH1 : (x > 0)) (PreH2 : (0 < num_pre)) (PreH3 : (num_pre <= INT_MAX)) (PreH4 : (0 <= x)) (PreH5 : (0 <= bits)) (PreH6 : (out = 0)) (PreH7 : (binary_safe_103 num_pre )) (PreH8 : (binary_count_state_z_103 num_pre x bits )) ,
+  ((( &( "num" ) )) # Int  |-> num_pre)
+  **  ((( &( "x" ) )) # Int  |-> x)
+  **  ((( &( "bits" ) )) # Int  |-> (bits + 1 ))
+  **  ((( &( "out" ) )) # Ptr  |-> out)
+|--
+  “ (2 <= INT_MAX) ” 
+  &&  “ ((INT_MIN) <= 2) ”
+.
+
+Definition to_binary_string_safety_wit_14 := 
+(
+forall (num_pre: Z) (x: Z) (bits: Z) (out: Z) (PreH1 : (0 < num_pre)) (PreH2 : (num_pre <= INT_MAX)) (PreH3 : (x = 0)) (PreH4 : (bits = (binary_length_z_103 (num_pre)))) (PreH5 : (1 <= bits)) (PreH6 : (out = 0)) (PreH7 : (binary_safe_103 num_pre )) ,
+  ((( &( "num" ) )) # Int  |-> num_pre)
+  **  ((( &( "x" ) )) # Int  |-> x)
+  **  ((( &( "bits" ) )) # Int  |-> bits)
+  **  ((( &( "out" ) )) # Ptr  |-> out)
+|--
+  “ ((bits + 1 ) <= INT_MAX) ” 
+  &&  “ ((INT_MIN) <= (bits + 1 )) ”
+) \/
+(
+forall (num_pre: Z) (x: Z) (bits: Z) (out: Z) (PreH1 : (0 < num_pre)) (PreH2 : (num_pre <= INT_MAX)) (PreH3 : (x = 0)) (PreH4 : (bits = (binary_length_z_103 (num_pre)))) (PreH5 : (1 <= bits)) (PreH6 : (out = 0)) (PreH7 : (binary_safe_103 num_pre )) ,
+  ((( &( "num" ) )) # Int  |-> num_pre)
+  **  ((( &( "x" ) )) # Int  |-> x)
+  **  ((( &( "bits" ) )) # Int  |-> bits)
+  **  ((( &( "out" ) )) # Ptr  |-> out)
+|--
+  “ ((bits + 1 ) <= INT_MAX) ” 
+  &&  “ ((INT_MIN) <= (bits + 1 )) ”
+).
+
+Definition to_binary_string_safety_wit_14_split_goal_1 := 
+forall (num_pre: Z) (x: Z) (bits: Z) (out: Z) (PreH1 : (0 < num_pre)) (PreH2 : (num_pre <= INT_MAX)) (PreH3 : (x = 0)) (PreH4 : (bits = (binary_length_z_103 (num_pre)))) (PreH5 : (1 <= bits)) (PreH6 : (out = 0)) (PreH7 : (binary_safe_103 num_pre )) ,
+  ((( &( "num" ) )) # Int  |-> num_pre)
+  **  ((( &( "x" ) )) # Int  |-> x)
+  **  ((( &( "bits" ) )) # Int  |-> bits)
+  **  ((( &( "out" ) )) # Ptr  |-> out)
+|--
+  “ ((bits + 1 ) <= INT_MAX) ”
+.
+
+Definition to_binary_string_safety_wit_14_split_goal_2 := 
+forall (num_pre: Z) (x: Z) (bits: Z) (out: Z) (PreH1 : (0 < num_pre)) (PreH2 : (num_pre <= INT_MAX)) (PreH3 : (x = 0)) (PreH4 : (bits = (binary_length_z_103 (num_pre)))) (PreH5 : (1 <= bits)) (PreH6 : (out = 0)) (PreH7 : (binary_safe_103 num_pre )) ,
+  ((( &( "num" ) )) # Int  |-> num_pre)
+  **  ((( &( "x" ) )) # Int  |-> x)
+  **  ((( &( "bits" ) )) # Int  |-> bits)
+  **  ((( &( "out" ) )) # Ptr  |-> out)
+|--
+  “ ((INT_MIN) <= (bits + 1 )) ”
+.
+
+Definition to_binary_string_safety_wit_15 := 
+forall (num_pre: Z) (x: Z) (bits: Z) (out: Z) (PreH1 : (0 < num_pre)) (PreH2 : (num_pre <= INT_MAX)) (PreH3 : (x = 0)) (PreH4 : (bits = (binary_length_z_103 (num_pre)))) (PreH5 : (1 <= bits)) (PreH6 : (out = 0)) (PreH7 : (binary_safe_103 num_pre )) ,
+  ((( &( "num" ) )) # Int  |-> num_pre)
+  **  ((( &( "x" ) )) # Int  |-> x)
+  **  ((( &( "bits" ) )) # Int  |-> bits)
+  **  ((( &( "out" ) )) # Ptr  |-> out)
+|--
+  “ (1 <= INT_MAX) ” 
+  &&  “ ((INT_MIN) <= 1) ”
+.
+
+Definition to_binary_string_safety_wit_16 := 
+forall (num_pre: Z) (x: Z) (bits: Z) (out: Z) (retval: Z) (PreH1 : (retval <> 0)) (PreH2 : (0 < num_pre)) (PreH3 : (num_pre <= INT_MAX)) (PreH4 : (x = 0)) (PreH5 : (bits = (binary_length_z_103 (num_pre)))) (PreH6 : (1 <= bits)) (PreH7 : (out = 0)) (PreH8 : (binary_safe_103 num_pre )) ,
+  (CharArray.undef_full retval (bits + 1 ) )
+  **  ((( &( "num" ) )) # Int  |-> num_pre)
+  **  ((( &( "x" ) )) # Int  |-> x)
+  **  ((( &( "bits" ) )) # Int  |-> bits)
+  **  ((( &( "out" ) )) # Ptr  |-> retval)
+|--
+  “ (0 <= INT_MAX) ” 
+  &&  “ ((INT_MIN) <= 0) ”
+.
+
+Definition to_binary_string_safety_wit_17 := 
+forall (num_pre: Z) (suffix: (@list Z)) (out: Z) (bits: Z) (x: Z) (num: Z) (PreH1 : (0 <= num)) (PreH2 : (num <= num_pre)) (PreH3 : (0 < num_pre)) (PreH4 : (num_pre <= INT_MAX)) (PreH5 : (x = 0)) (PreH6 : (0 <= bits)) (PreH7 : (bits <= (binary_length_z_103 (num_pre)))) (PreH8 : (out <> 0)) (PreH9 : (binary_safe_103 num_pre )) (PreH10 : (binary_backfill_state_z_103 num_pre num bits suffix )) (PreH11 : ((Zlength (suffix)) = (((binary_length_z_103 (num_pre)) + 1 ) - bits ))) ,
+  ((( &( "num" ) )) # Int  |-> num)
+  **  ((( &( "x" ) )) # Int  |-> x)
+  **  ((( &( "bits" ) )) # Int  |-> bits)
+  **  ((( &( "out" ) )) # Ptr  |-> out)
+  **  (CharArray.undef_seg out 0 bits )
+  **  (CharArray.seg out bits ((binary_length_z_103 (num_pre)) + 1 ) suffix )
+|--
+  “ (0 <= INT_MAX) ” 
+  &&  “ ((INT_MIN) <= 0) ”
+.
+
+Definition to_binary_string_safety_wit_18 := 
+forall (num_pre: Z) (suffix: (@list Z)) (num: Z) (x: Z) (bits: Z) (out: Z) (PreH1 : (0 < num)) (PreH2 : (num <= num_pre)) (PreH3 : (0 < num_pre)) (PreH4 : (num_pre <= INT_MAX)) (PreH5 : (x = 0)) (PreH6 : (0 < bits)) (PreH7 : (bits <= (binary_length_z_103 (num_pre)))) (PreH8 : (out <> 0)) (PreH9 : (binary_safe_103 num_pre )) (PreH10 : (binary_backfill_state_z_103 num_pre num bits suffix )) (PreH11 : ((Zlength (suffix)) = (((binary_length_z_103 (num_pre)) + 1 ) - bits ))) ,
+  ((( &( "num" ) )) # Int  |-> num)
+  **  ((( &( "x" ) )) # Int  |-> x)
+  **  ((( &( "bits" ) )) # Int  |-> bits)
+  **  ((( &( "out" ) )) # Ptr  |-> out)
+  **  (CharArray.undef_seg out 0 bits )
+  **  (CharArray.seg out bits ((binary_length_z_103 (num_pre)) + 1 ) suffix )
+|--
+  “ ((bits - 1 ) <= INT_MAX) ” 
+  &&  “ ((INT_MIN) <= (bits - 1 )) ”
+.
+
+Definition to_binary_string_safety_wit_19 := 
+forall (num_pre: Z) (suffix: (@list Z)) (num: Z) (x: Z) (bits: Z) (out: Z) (PreH1 : (0 < num)) (PreH2 : (num <= num_pre)) (PreH3 : (0 < num_pre)) (PreH4 : (num_pre <= INT_MAX)) (PreH5 : (x = 0)) (PreH6 : (0 < bits)) (PreH7 : (bits <= (binary_length_z_103 (num_pre)))) (PreH8 : (out <> 0)) (PreH9 : (binary_safe_103 num_pre )) (PreH10 : (binary_backfill_state_z_103 num_pre num bits suffix )) (PreH11 : ((Zlength (suffix)) = (((binary_length_z_103 (num_pre)) + 1 ) - bits ))) ,
+  ((( &( "num" ) )) # Int  |-> num)
+  **  ((( &( "x" ) )) # Int  |-> x)
+  **  ((( &( "bits" ) )) # Int  |-> bits)
+  **  ((( &( "out" ) )) # Ptr  |-> out)
+  **  (CharArray.undef_seg out 0 bits )
+  **  (CharArray.seg out bits ((binary_length_z_103 (num_pre)) + 1 ) suffix )
+|--
+  “ (1 <= INT_MAX) ” 
+  &&  “ ((INT_MIN) <= 1) ”
+.
+
+Definition to_binary_string_safety_wit_20 := 
+(
+forall (num_pre: Z) (suffix: (@list Z)) (num: Z) (x: Z) (bits: Z) (out: Z) (PreH1 : (0 < num)) (PreH2 : (num <= num_pre)) (PreH3 : (0 < num_pre)) (PreH4 : (num_pre <= INT_MAX)) (PreH5 : (x = 0)) (PreH6 : (0 < bits)) (PreH7 : (bits <= (binary_length_z_103 (num_pre)))) (PreH8 : (out <> 0)) (PreH9 : (binary_safe_103 num_pre )) (PreH10 : (binary_backfill_state_z_103 num_pre num bits suffix )) (PreH11 : ((Zlength (suffix)) = (((binary_length_z_103 (num_pre)) + 1 ) - bits ))) ,
+  ((( &( "num" ) )) # Int  |-> num)
+  **  ((( &( "x" ) )) # Int  |-> x)
+  **  ((( &( "bits" ) )) # Int  |-> bits)
+  **  ((( &( "out" ) )) # Ptr  |-> out)
+  **  (CharArray.undef_seg out 0 bits )
+  **  (CharArray.seg out bits ((binary_length_z_103 (num_pre)) + 1 ) suffix )
+|--
+  “ ((48 + (num % ( 2 ) ) ) <= INT_MAX) ” 
+  &&  “ ((INT_MIN) <= (48 + (num % ( 2 ) ) )) ”
+) \/
+(
+forall (num_pre: Z) (suffix: (@list Z)) (num: Z) (x: Z) (bits: Z) (out: Z) (PreH1 : (0 < num)) (PreH2 : (num <= num_pre)) (PreH3 : (0 < num_pre)) (PreH4 : (num_pre <= INT_MAX)) (PreH5 : (x = 0)) (PreH6 : (0 < bits)) (PreH7 : (bits <= (binary_length_z_103 (num_pre)))) (PreH8 : (out <> 0)) (PreH9 : (binary_safe_103 num_pre )) (PreH10 : (binary_backfill_state_z_103 num_pre num bits suffix )) (PreH11 : ((Zlength (suffix)) = (((binary_length_z_103 (num_pre)) + 1 ) - bits ))) ,
+  ((( &( "num" ) )) # Int  |-> num)
+  **  ((( &( "x" ) )) # Int  |-> x)
+  **  ((( &( "bits" ) )) # Int  |-> bits)
+  **  ((( &( "out" ) )) # Ptr  |-> out)
+  **  (CharArray.undef_seg out 0 bits )
+  **  (CharArray.seg out bits ((binary_length_z_103 (num_pre)) + 1 ) suffix )
+|--
+  “ ((48 + (num % ( 2 ) ) ) <= INT_MAX) ” 
+  &&  “ ((INT_MIN) <= (48 + (num % ( 2 ) ) )) ”
+).
+
+Definition to_binary_string_safety_wit_20_split_goal_1 := 
+forall (num_pre: Z) (suffix: (@list Z)) (num: Z) (x: Z) (bits: Z) (out: Z) (PreH1 : (0 < num)) (PreH2 : (num <= num_pre)) (PreH3 : (0 < num_pre)) (PreH4 : (num_pre <= INT_MAX)) (PreH5 : (x = 0)) (PreH6 : (0 < bits)) (PreH7 : (bits <= (binary_length_z_103 (num_pre)))) (PreH8 : (out <> 0)) (PreH9 : (binary_safe_103 num_pre )) (PreH10 : (binary_backfill_state_z_103 num_pre num bits suffix )) (PreH11 : ((Zlength (suffix)) = (((binary_length_z_103 (num_pre)) + 1 ) - bits ))) ,
+  ((( &( "num" ) )) # Int  |-> num)
+  **  ((( &( "x" ) )) # Int  |-> x)
+  **  ((( &( "bits" ) )) # Int  |-> bits)
+  **  ((( &( "out" ) )) # Ptr  |-> out)
+  **  (CharArray.undef_seg out 0 bits )
+  **  (CharArray.seg out bits ((binary_length_z_103 (num_pre)) + 1 ) suffix )
+|--
+  “ ((48 + (num % ( 2 ) ) ) <= INT_MAX) ”
+.
+
+Definition to_binary_string_safety_wit_20_split_goal_2 := 
+forall (num_pre: Z) (suffix: (@list Z)) (num: Z) (x: Z) (bits: Z) (out: Z) (PreH1 : (0 < num)) (PreH2 : (num <= num_pre)) (PreH3 : (0 < num_pre)) (PreH4 : (num_pre <= INT_MAX)) (PreH5 : (x = 0)) (PreH6 : (0 < bits)) (PreH7 : (bits <= (binary_length_z_103 (num_pre)))) (PreH8 : (out <> 0)) (PreH9 : (binary_safe_103 num_pre )) (PreH10 : (binary_backfill_state_z_103 num_pre num bits suffix )) (PreH11 : ((Zlength (suffix)) = (((binary_length_z_103 (num_pre)) + 1 ) - bits ))) ,
+  ((( &( "num" ) )) # Int  |-> num)
+  **  ((( &( "x" ) )) # Int  |-> x)
+  **  ((( &( "bits" ) )) # Int  |-> bits)
+  **  ((( &( "out" ) )) # Ptr  |-> out)
+  **  (CharArray.undef_seg out 0 bits )
+  **  (CharArray.seg out bits ((binary_length_z_103 (num_pre)) + 1 ) suffix )
+|--
+  “ ((INT_MIN) <= (48 + (num % ( 2 ) ) )) ”
+.
+
+Definition to_binary_string_safety_wit_21 := 
+forall (num_pre: Z) (suffix: (@list Z)) (num: Z) (x: Z) (bits: Z) (out: Z) (PreH1 : (0 < num)) (PreH2 : (num <= num_pre)) (PreH3 : (0 < num_pre)) (PreH4 : (num_pre <= INT_MAX)) (PreH5 : (x = 0)) (PreH6 : (0 < bits)) (PreH7 : (bits <= (binary_length_z_103 (num_pre)))) (PreH8 : (out <> 0)) (PreH9 : (binary_safe_103 num_pre )) (PreH10 : (binary_backfill_state_z_103 num_pre num bits suffix )) (PreH11 : ((Zlength (suffix)) = (((binary_length_z_103 (num_pre)) + 1 ) - bits ))) ,
+  ((( &( "num" ) )) # Int  |-> num)
+  **  ((( &( "x" ) )) # Int  |-> x)
+  **  ((( &( "bits" ) )) # Int  |-> bits)
+  **  ((( &( "out" ) )) # Ptr  |-> out)
+  **  (CharArray.undef_seg out 0 bits )
+  **  (CharArray.seg out bits ((binary_length_z_103 (num_pre)) + 1 ) suffix )
+|--
+  “ ((num <> (INT_MIN)) \/ (2 <> (-1))) ” 
+  &&  “ (2 <> 0) ”
+.
+
+Definition to_binary_string_safety_wit_22 := 
+forall (num_pre: Z) (suffix: (@list Z)) (num: Z) (x: Z) (bits: Z) (out: Z) (PreH1 : (0 < num)) (PreH2 : (num <= num_pre)) (PreH3 : (0 < num_pre)) (PreH4 : (num_pre <= INT_MAX)) (PreH5 : (x = 0)) (PreH6 : (0 < bits)) (PreH7 : (bits <= (binary_length_z_103 (num_pre)))) (PreH8 : (out <> 0)) (PreH9 : (binary_safe_103 num_pre )) (PreH10 : (binary_backfill_state_z_103 num_pre num bits suffix )) (PreH11 : ((Zlength (suffix)) = (((binary_length_z_103 (num_pre)) + 1 ) - bits ))) ,
+  ((( &( "num" ) )) # Int  |-> num)
+  **  ((( &( "x" ) )) # Int  |-> x)
+  **  ((( &( "bits" ) )) # Int  |-> bits)
+  **  ((( &( "out" ) )) # Ptr  |-> out)
+  **  (CharArray.undef_seg out 0 bits )
+  **  (CharArray.seg out bits ((binary_length_z_103 (num_pre)) + 1 ) suffix )
+|--
+  “ (48 <= INT_MAX) ” 
+  &&  “ ((INT_MIN) <= 48) ”
+.
+
+Definition to_binary_string_safety_wit_23 := 
+forall (num_pre: Z) (suffix: (@list Z)) (num: Z) (x: Z) (bits: Z) (out: Z) (PreH1 : (0 < num)) (PreH2 : (num <= num_pre)) (PreH3 : (0 < num_pre)) (PreH4 : (num_pre <= INT_MAX)) (PreH5 : (x = 0)) (PreH6 : (0 < bits)) (PreH7 : (bits <= (binary_length_z_103 (num_pre)))) (PreH8 : (out <> 0)) (PreH9 : (binary_safe_103 num_pre )) (PreH10 : (binary_backfill_state_z_103 num_pre num bits suffix )) (PreH11 : ((Zlength (suffix)) = (((binary_length_z_103 (num_pre)) + 1 ) - bits ))) ,
+  ((( &( "num" ) )) # Int  |-> num)
+  **  ((( &( "x" ) )) # Int  |-> x)
+  **  ((( &( "bits" ) )) # Int  |-> bits)
+  **  ((( &( "out" ) )) # Ptr  |-> out)
+  **  (CharArray.undef_seg out 0 bits )
+  **  (CharArray.seg out bits ((binary_length_z_103 (num_pre)) + 1 ) suffix )
+|--
+  “ (2 <= INT_MAX) ” 
+  &&  “ ((INT_MIN) <= 2) ”
+.
+
+Definition to_binary_string_safety_wit_24 := 
+forall (num_pre: Z) (suffix: (@list Z)) (num: Z) (x: Z) (bits: Z) (out: Z) (PreH1 : (0 < num)) (PreH2 : (num <= num_pre)) (PreH3 : (0 < num_pre)) (PreH4 : (num_pre <= INT_MAX)) (PreH5 : (x = 0)) (PreH6 : (0 < bits)) (PreH7 : (bits <= (binary_length_z_103 (num_pre)))) (PreH8 : (out <> 0)) (PreH9 : (binary_safe_103 num_pre )) (PreH10 : (binary_backfill_state_z_103 num_pre (num ÷ 2 ) (bits - 1 ) (cons ((48 + (num % ( 2 ) ) )) (suffix)) )) (PreH11 : ((Zlength ((cons ((48 + (num % ( 2 ) ) )) (suffix)))) = (((binary_length_z_103 (num_pre)) + 1 ) - (bits - 1 ) ))) ,
+  ((( &( "num" ) )) # Int  |-> num)
+  **  ((( &( "x" ) )) # Int  |-> x)
+  **  ((( &( "bits" ) )) # Int  |-> bits)
+  **  ((( &( "out" ) )) # Ptr  |-> out)
+  **  (CharArray.undef_seg out 0 (bits - 1 ) )
+  **  (CharArray.seg out (bits - 1 ) ((binary_length_z_103 (num_pre)) + 1 ) (cons ((48 + (num % ( 2 ) ) )) (suffix)) )
+|--
+  “ ((bits - 1 ) <= INT_MAX) ” 
+  &&  “ ((INT_MIN) <= (bits - 1 )) ”
+.
+
+Definition to_binary_string_safety_wit_25 := 
+forall (num_pre: Z) (suffix: (@list Z)) (num: Z) (x: Z) (bits: Z) (out: Z) (PreH1 : (0 < num)) (PreH2 : (num <= num_pre)) (PreH3 : (0 < num_pre)) (PreH4 : (num_pre <= INT_MAX)) (PreH5 : (x = 0)) (PreH6 : (0 < bits)) (PreH7 : (bits <= (binary_length_z_103 (num_pre)))) (PreH8 : (out <> 0)) (PreH9 : (binary_safe_103 num_pre )) (PreH10 : (binary_backfill_state_z_103 num_pre (num ÷ 2 ) (bits - 1 ) (cons ((48 + (num % ( 2 ) ) )) (suffix)) )) (PreH11 : ((Zlength ((cons ((48 + (num % ( 2 ) ) )) (suffix)))) = (((binary_length_z_103 (num_pre)) + 1 ) - (bits - 1 ) ))) ,
+  ((( &( "num" ) )) # Int  |-> num)
+  **  ((( &( "x" ) )) # Int  |-> x)
+  **  ((( &( "bits" ) )) # Int  |-> bits)
+  **  ((( &( "out" ) )) # Ptr  |-> out)
+  **  (CharArray.undef_seg out 0 (bits - 1 ) )
+  **  (CharArray.seg out (bits - 1 ) ((binary_length_z_103 (num_pre)) + 1 ) (cons ((48 + (num % ( 2 ) ) )) (suffix)) )
+|--
+  “ (1 <= INT_MAX) ” 
+  &&  “ ((INT_MIN) <= 1) ”
+.
+
+Definition to_binary_string_safety_wit_26 := 
+forall (num_pre: Z) (suffix: (@list Z)) (num: Z) (x: Z) (bits: Z) (out: Z) (PreH1 : (0 < num)) (PreH2 : (num <= num_pre)) (PreH3 : (0 < num_pre)) (PreH4 : (num_pre <= INT_MAX)) (PreH5 : (x = 0)) (PreH6 : (0 < bits)) (PreH7 : (bits <= (binary_length_z_103 (num_pre)))) (PreH8 : (out <> 0)) (PreH9 : (binary_safe_103 num_pre )) (PreH10 : (binary_backfill_state_z_103 num_pre (num ÷ 2 ) (bits - 1 ) (cons ((48 + (num % ( 2 ) ) )) (suffix)) )) (PreH11 : ((Zlength ((cons ((48 + (num % ( 2 ) ) )) (suffix)))) = (((binary_length_z_103 (num_pre)) + 1 ) - (bits - 1 ) ))) ,
+  ((( &( "num" ) )) # Int  |-> num)
+  **  ((( &( "x" ) )) # Int  |-> x)
+  **  ((( &( "bits" ) )) # Int  |-> (bits - 1 ))
+  **  ((( &( "out" ) )) # Ptr  |-> out)
+  **  (CharArray.undef_seg out 0 (bits - 1 ) )
+  **  (CharArray.seg out (bits - 1 ) ((binary_length_z_103 (num_pre)) + 1 ) (cons ((48 + (num % ( 2 ) ) )) (suffix)) )
+|--
+  “ ((num <> (INT_MIN)) \/ (2 <> (-1))) ” 
+  &&  “ (2 <> 0) ”
+.
+
+Definition to_binary_string_safety_wit_27 := 
+forall (num_pre: Z) (suffix: (@list Z)) (num: Z) (x: Z) (bits: Z) (out: Z) (PreH1 : (0 < num)) (PreH2 : (num <= num_pre)) (PreH3 : (0 < num_pre)) (PreH4 : (num_pre <= INT_MAX)) (PreH5 : (x = 0)) (PreH6 : (0 < bits)) (PreH7 : (bits <= (binary_length_z_103 (num_pre)))) (PreH8 : (out <> 0)) (PreH9 : (binary_safe_103 num_pre )) (PreH10 : (binary_backfill_state_z_103 num_pre (num ÷ 2 ) (bits - 1 ) (cons ((48 + (num % ( 2 ) ) )) (suffix)) )) (PreH11 : ((Zlength ((cons ((48 + (num % ( 2 ) ) )) (suffix)))) = (((binary_length_z_103 (num_pre)) + 1 ) - (bits - 1 ) ))) ,
+  ((( &( "num" ) )) # Int  |-> num)
+  **  ((( &( "x" ) )) # Int  |-> x)
+  **  ((( &( "bits" ) )) # Int  |-> (bits - 1 ))
+  **  ((( &( "out" ) )) # Ptr  |-> out)
+  **  (CharArray.undef_seg out 0 (bits - 1 ) )
+  **  (CharArray.seg out (bits - 1 ) ((binary_length_z_103 (num_pre)) + 1 ) (cons ((48 + (num % ( 2 ) ) )) (suffix)) )
+|--
+  “ (2 <= INT_MAX) ” 
+  &&  “ ((INT_MIN) <= 2) ”
+.
+
+Definition to_binary_string_entail_wit_1 := 
+(
+forall (num_pre: Z) (PreH1 : (num_pre <> 0)) (PreH2 : (0 <= num_pre)) (PreH3 : (num_pre <= INT_MAX)) (PreH4 : (binary_safe_103 num_pre )) ,
+  TT && emp 
+|--
+  “ (0 < num_pre) ” 
+  &&  “ (num_pre <= INT_MAX) ” 
+  &&  “ (0 <= num_pre) ” 
+  &&  “ (0 <= 0) ” 
+  &&  “ (0 = 0) ” 
+  &&  “ (binary_safe_103 num_pre ) ” 
+  &&  “ (binary_count_state_z_103 num_pre num_pre 0 ) ”
+  &&  emp
+) \/
+(
+forall (num_pre: Z) (PreH1 : (num_pre <> 0)) (PreH2 : (0 <= num_pre)) (PreH3 : (num_pre <= INT_MAX)) (PreH4 : (binary_safe_103 num_pre )) ,
+  TT && emp 
+|--
+  “ (binary_count_state_z_103 num_pre num_pre 0 ) ”
+  &&  emp
+).
+
+Definition to_binary_string_entail_wit_1_split_goal_1 := 
+forall (num_pre: Z) (PreH1 : (num_pre <> 0)) (PreH2 : (0 <= num_pre)) (PreH3 : (num_pre <= INT_MAX)) (PreH4 : (binary_safe_103 num_pre )) ,
+  TT && emp 
+|--
+  “ (binary_count_state_z_103 num_pre num_pre 0 ) ”
+.
+
+Definition to_binary_string_entail_wit_2 := 
+(
+forall (num_pre: Z) (out: Z) (bits: Z) (x: Z) (PreH1 : (x > 0)) (PreH2 : (0 < num_pre)) (PreH3 : (num_pre <= INT_MAX)) (PreH4 : (0 <= x)) (PreH5 : (0 <= bits)) (PreH6 : (out = 0)) (PreH7 : (binary_safe_103 num_pre )) (PreH8 : (binary_count_state_z_103 num_pre x bits )) ,
+  TT && emp 
+|--
+  “ (0 < num_pre) ” 
+  &&  “ (num_pre <= INT_MAX) ” 
+  &&  “ (0 <= (x ÷ 2 )) ” 
+  &&  “ (0 <= (bits + 1 )) ” 
+  &&  “ (out = 0) ” 
+  &&  “ (binary_safe_103 num_pre ) ” 
+  &&  “ (binary_count_state_z_103 num_pre (x ÷ 2 ) (bits + 1 ) ) ”
+  &&  emp
+) \/
+(
+forall (num_pre: Z) (out: Z) (bits: Z) (x: Z) (PreH1 : (x > 0)) (PreH2 : (0 < num_pre)) (PreH3 : (num_pre <= INT_MAX)) (PreH4 : (0 <= x)) (PreH5 : (0 <= bits)) (PreH6 : (out = 0)) (PreH7 : (binary_safe_103 num_pre )) (PreH8 : (binary_count_state_z_103 num_pre x bits )) ,
+  TT && emp 
+|--
+  “ (binary_count_state_z_103 num_pre (x ÷ 2 ) (bits + 1 ) ) ” 
+  &&  “ (0 <= (x ÷ 2 )) ”
+  &&  emp
+).
+
+Definition to_binary_string_entail_wit_2_split_goal_1 := 
+forall (num_pre: Z) (out: Z) (bits: Z) (x: Z) (PreH1 : (x > 0)) (PreH2 : (0 < num_pre)) (PreH3 : (num_pre <= INT_MAX)) (PreH4 : (0 <= x)) (PreH5 : (0 <= bits)) (PreH6 : (out = 0)) (PreH7 : (binary_safe_103 num_pre )) (PreH8 : (binary_count_state_z_103 num_pre x bits )) ,
+  TT && emp 
+|--
+  “ (binary_count_state_z_103 num_pre (x ÷ 2 ) (bits + 1 ) ) ”
+.
+
+Definition to_binary_string_entail_wit_2_split_goal_2 := 
+forall (num_pre: Z) (out: Z) (bits: Z) (x: Z) (PreH1 : (x > 0)) (PreH2 : (0 < num_pre)) (PreH3 : (num_pre <= INT_MAX)) (PreH4 : (0 <= x)) (PreH5 : (0 <= bits)) (PreH6 : (out = 0)) (PreH7 : (binary_safe_103 num_pre )) (PreH8 : (binary_count_state_z_103 num_pre x bits )) ,
+  TT && emp 
+|--
+  “ (0 <= (x ÷ 2 )) ”
+.
+
+Definition to_binary_string_entail_wit_3 := 
+(
+forall (num_pre: Z) (out: Z) (bits: Z) (x: Z) (PreH1 : (x <= 0)) (PreH2 : (0 < num_pre)) (PreH3 : (num_pre <= INT_MAX)) (PreH4 : (0 <= x)) (PreH5 : (0 <= bits)) (PreH6 : (out = 0)) (PreH7 : (binary_safe_103 num_pre )) (PreH8 : (binary_count_state_z_103 num_pre x bits )) ,
+  TT && emp 
+|--
+  “ (0 < num_pre) ” 
+  &&  “ (num_pre <= INT_MAX) ” 
+  &&  “ (x = 0) ” 
+  &&  “ (bits = (binary_length_z_103 (num_pre))) ” 
+  &&  “ (1 <= bits) ” 
+  &&  “ (out = 0) ” 
+  &&  “ (binary_safe_103 num_pre ) ”
+  &&  emp
+) \/
+(
+forall (num_pre: Z) (out: Z) (bits: Z) (x: Z) (PreH1 : (x <= 0)) (PreH2 : (0 < num_pre)) (PreH3 : (num_pre <= INT_MAX)) (PreH4 : (0 <= x)) (PreH5 : (0 <= bits)) (PreH6 : (out = 0)) (PreH7 : (binary_safe_103 num_pre )) (PreH8 : (binary_count_state_z_103 num_pre x bits )) ,
+  TT && emp 
+|--
+  “ (1 <= bits) ” 
+  &&  “ (bits = (binary_length_z_103 (num_pre))) ”
+  &&  emp
+).
+
+Definition to_binary_string_entail_wit_3_split_goal_1 := 
+forall (num_pre: Z) (out: Z) (bits: Z) (x: Z) (PreH1 : (x <= 0)) (PreH2 : (0 < num_pre)) (PreH3 : (num_pre <= INT_MAX)) (PreH4 : (0 <= x)) (PreH5 : (0 <= bits)) (PreH6 : (out = 0)) (PreH7 : (binary_safe_103 num_pre )) (PreH8 : (binary_count_state_z_103 num_pre x bits )) ,
+  TT && emp 
+|--
+  “ (1 <= bits) ”
+.
+
+Definition to_binary_string_entail_wit_3_split_goal_2 := 
+forall (num_pre: Z) (out: Z) (bits: Z) (x: Z) (PreH1 : (x <= 0)) (PreH2 : (0 < num_pre)) (PreH3 : (num_pre <= INT_MAX)) (PreH4 : (0 <= x)) (PreH5 : (0 <= bits)) (PreH6 : (out = 0)) (PreH7 : (binary_safe_103 num_pre )) (PreH8 : (binary_count_state_z_103 num_pre x bits )) ,
+  TT && emp 
+|--
+  “ (bits = (binary_length_z_103 (num_pre))) ”
+.
+
+Definition to_binary_string_entail_wit_4 := 
+(
+forall (num_pre: Z) (x: Z) (bits: Z) (out: Z) (retval: Z) (PreH1 : (retval <> 0)) (PreH2 : (0 < num_pre)) (PreH3 : (num_pre <= INT_MAX)) (PreH4 : (x = 0)) (PreH5 : (bits = (binary_length_z_103 (num_pre)))) (PreH6 : (1 <= bits)) (PreH7 : (out = 0)) (PreH8 : (binary_safe_103 num_pre )) ,
+  (((retval + (bits * sizeof(CHAR) ) )) # Char  |-> 0)
+  **  (CharArray.undef_missing_i retval bits 0 (bits + 1 ) )
+|--
+  “ (0 < num_pre) ” 
+  &&  “ (num_pre <= INT_MAX) ” 
+  &&  “ (x = 0) ” 
+  &&  “ (bits = (binary_length_z_103 (num_pre))) ” 
+  &&  “ (1 <= bits) ” 
+  &&  “ (retval <> 0) ” 
+  &&  “ (binary_safe_103 num_pre ) ” 
+  &&  “ (binary_backfill_state_z_103 num_pre num_pre bits (cons (0) ((@nil Z))) ) ”
+  &&  (CharArray.undef_seg retval 0 bits )
+  **  (CharArray.seg retval bits (bits + 1 ) (cons (0) ((@nil Z))) )
+) \/
+(
+forall (num_pre: Z) (x: Z) (bits: Z) (out: Z) (retval: Z) (PreH1 : (retval <> 0)) (PreH2 : (0 < num_pre)) (PreH3 : (num_pre <= INT_MAX)) (PreH4 : (x = 0)) (PreH5 : (bits = (binary_length_z_103 (num_pre)))) (PreH6 : (1 <= bits)) (PreH7 : (out = 0)) (PreH8 : (binary_safe_103 num_pre )) ,
+  (((retval + (bits * sizeof(CHAR) ) )) # Char  |-> 0)
+  **  (CharArray.undef_missing_i retval bits 0 (bits + 1 ) )
+|--
+  “ (binary_backfill_state_z_103 num_pre num_pre bits (cons (0) ((@nil Z))) ) ”
+  &&  (CharArray.undef_full retval bits )
+  **  (CharArray.seg retval bits (bits + 1 ) (cons (0) ((@nil Z))) )
+).
+
+Definition to_binary_string_entail_wit_4_split_goal_1 := 
+forall (num_pre: Z) (x: Z) (bits: Z) (out: Z) (retval: Z) (PreH1 : (retval <> 0)) (PreH2 : (0 < num_pre)) (PreH3 : (num_pre <= INT_MAX)) (PreH4 : (x = 0)) (PreH5 : (bits = (binary_length_z_103 (num_pre)))) (PreH6 : (1 <= bits)) (PreH7 : (out = 0)) (PreH8 : (binary_safe_103 num_pre )) ,
+  (((retval + (bits * sizeof(CHAR) ) )) # Char  |-> 0)
+  **  (CharArray.undef_missing_i retval bits 0 (bits + 1 ) )
+|--
+  “ (binary_backfill_state_z_103 num_pre num_pre bits (cons (0) ((@nil Z))) ) ”
+.
+
+Definition to_binary_string_entail_wit_4_split_goal_spatial := 
+forall (num_pre: Z) (x: Z) (bits: Z) (out: Z) (retval: Z) (PreH1 : (retval <> 0)) (PreH2 : (0 < num_pre)) (PreH3 : (num_pre <= INT_MAX)) (PreH4 : (x = 0)) (PreH5 : (bits = (binary_length_z_103 (num_pre)))) (PreH6 : (1 <= bits)) (PreH7 : (out = 0)) (PreH8 : (binary_safe_103 num_pre )) ,
+  (((retval + (bits * sizeof(CHAR) ) )) # Char  |-> 0)
+  **  (CharArray.undef_missing_i retval bits 0 (bits + 1 ) )
+|--
+  (CharArray.undef_full retval bits )
+  **  (CharArray.seg retval bits (bits + 1 ) (cons (0) ((@nil Z))) )
+.
+
+Definition to_binary_string_entail_wit_5 := 
+(
+forall (num_pre: Z) (x: Z) (bits: Z) (out: Z) (PreH1 : (0 < num_pre)) (PreH2 : (num_pre <= INT_MAX)) (PreH3 : (x = 0)) (PreH4 : (bits = (binary_length_z_103 (num_pre)))) (PreH5 : (1 <= bits)) (PreH6 : (out <> 0)) (PreH7 : (binary_safe_103 num_pre )) (PreH8 : (binary_backfill_state_z_103 num_pre num_pre bits (cons (0) ((@nil Z))) )) ,
+  (CharArray.undef_seg out 0 bits )
+  **  (CharArray.seg out bits (bits + 1 ) (cons (0) ((@nil Z))) )
+|--
+  EX (suffix: (@list Z)) ,
+  “ (0 <= num_pre) ” 
+  &&  “ (num_pre <= num_pre) ” 
+  &&  “ (0 < num_pre) ” 
+  &&  “ (num_pre <= INT_MAX) ” 
+  &&  “ (x = 0) ” 
+  &&  “ (0 <= bits) ” 
+  &&  “ (bits <= (binary_length_z_103 (num_pre))) ” 
+  &&  “ (out <> 0) ” 
+  &&  “ (binary_safe_103 num_pre ) ” 
+  &&  “ (binary_backfill_state_z_103 num_pre num_pre bits suffix ) ” 
+  &&  “ ((Zlength (suffix)) = (((binary_length_z_103 (num_pre)) + 1 ) - bits )) ”
+  &&  (CharArray.undef_seg out 0 bits )
+  **  (CharArray.seg out bits ((binary_length_z_103 (num_pre)) + 1 ) suffix )
+) \/
+(
+forall (num_pre: Z) (x: Z) (bits: Z) (out: Z) (PreH1 : (0 < num_pre)) (PreH2 : (num_pre <= INT_MAX)) (PreH3 : (x = 0)) (PreH4 : (bits = (binary_length_z_103 (num_pre)))) (PreH5 : (1 <= bits)) (PreH6 : (out <> 0)) (PreH7 : (binary_safe_103 num_pre )) (PreH8 : (binary_backfill_state_z_103 num_pre num_pre bits (cons (0) ((@nil Z))) )) ,
+  (CharArray.undef_seg out 0 bits )
+  **  (CharArray.seg out bits (bits + 1 ) (cons (0) ((@nil Z))) )
+|--
+  EX (suffix: (@list Z)) ,
+  “ (0 <= num_pre) ” 
+  &&  “ (num_pre <= num_pre) ” 
+  &&  “ (0 < num_pre) ” 
+  &&  “ (num_pre <= INT_MAX) ” 
+  &&  “ (x = 0) ” 
+  &&  “ (0 <= bits) ” 
+  &&  “ (bits <= (binary_length_z_103 (num_pre))) ” 
+  &&  “ (out <> 0) ” 
+  &&  “ (binary_safe_103 num_pre ) ” 
+  &&  “ (binary_backfill_state_z_103 num_pre num_pre bits suffix ) ” 
+  &&  “ ((Zlength (suffix)) = (((binary_length_z_103 (num_pre)) + 1 ) - bits )) ”
+  &&  (CharArray.undef_full out bits )
+  **  (CharArray.seg out bits ((binary_length_z_103 (num_pre)) + 1 ) suffix )
+).
+
+Definition to_binary_string_entail_wit_6 := 
+(
+forall (num_pre: Z) (suffix_2: (@list Z)) (out: Z) (bits: Z) (x: Z) (num: Z) (PreH1 : (num > 0)) (PreH2 : (0 <= num)) (PreH3 : (num <= num_pre)) (PreH4 : (0 < num_pre)) (PreH5 : (num_pre <= INT_MAX)) (PreH6 : (x = 0)) (PreH7 : (0 <= bits)) (PreH8 : (bits <= (binary_length_z_103 (num_pre)))) (PreH9 : (out <> 0)) (PreH10 : (binary_safe_103 num_pre )) (PreH11 : (binary_backfill_state_z_103 num_pre num bits suffix_2 )) (PreH12 : ((Zlength (suffix_2)) = (((binary_length_z_103 (num_pre)) + 1 ) - bits ))) ,
+  (CharArray.undef_seg out 0 bits )
+  **  (CharArray.seg out bits ((binary_length_z_103 (num_pre)) + 1 ) suffix_2 )
+|--
+  EX (suffix: (@list Z)) ,
+  “ (0 < num) ” 
+  &&  “ (num <= num_pre) ” 
+  &&  “ (0 < num_pre) ” 
+  &&  “ (num_pre <= INT_MAX) ” 
+  &&  “ (x = 0) ” 
+  &&  “ (0 < bits) ” 
+  &&  “ (bits <= (binary_length_z_103 (num_pre))) ” 
+  &&  “ (out <> 0) ” 
+  &&  “ (binary_safe_103 num_pre ) ” 
+  &&  “ (binary_backfill_state_z_103 num_pre num bits suffix ) ” 
+  &&  “ ((Zlength (suffix)) = (((binary_length_z_103 (num_pre)) + 1 ) - bits )) ”
+  &&  (CharArray.undef_seg out 0 bits )
+  **  (CharArray.seg out bits ((binary_length_z_103 (num_pre)) + 1 ) suffix )
+) \/
+(
+forall (num_pre: Z) (suffix_2: (@list Z)) (out: Z) (bits: Z) (x: Z) (num: Z) (PreH1 : (num > 0)) (PreH2 : (0 <= num)) (PreH3 : (num <= num_pre)) (PreH4 : (0 < num_pre)) (PreH5 : (num_pre <= INT_MAX)) (PreH6 : (x = 0)) (PreH7 : (0 <= bits)) (PreH8 : (bits <= (binary_length_z_103 (num_pre)))) (PreH9 : (out <> 0)) (PreH10 : (binary_safe_103 num_pre )) (PreH11 : (binary_backfill_state_z_103 num_pre num bits suffix_2 )) (PreH12 : ((Zlength (suffix_2)) = (((binary_length_z_103 (num_pre)) + 1 ) - bits ))) ,
+  (CharArray.undef_seg out 0 bits )
+|--
+  “ (0 < bits) ”
+  &&  (CharArray.undef_full out bits )
+).
+
+Definition to_binary_string_entail_wit_6_split_goal_1 := 
+forall (num_pre: Z) (suffix_2: (@list Z)) (out: Z) (bits: Z) (x: Z) (num: Z) (PreH1 : (num > 0)) (PreH2 : (0 <= num)) (PreH3 : (num <= num_pre)) (PreH4 : (0 < num_pre)) (PreH5 : (num_pre <= INT_MAX)) (PreH6 : (x = 0)) (PreH7 : (0 <= bits)) (PreH8 : (bits <= (binary_length_z_103 (num_pre)))) (PreH9 : (out <> 0)) (PreH10 : (binary_safe_103 num_pre )) (PreH11 : (binary_backfill_state_z_103 num_pre num bits suffix_2 )) (PreH12 : ((Zlength (suffix_2)) = (((binary_length_z_103 (num_pre)) + 1 ) - bits ))) ,
+  (CharArray.undef_seg out 0 bits )
+|--
+  “ (0 < bits) ”
+.
+
+Definition to_binary_string_entail_wit_6_split_goal_spatial := 
+forall (num_pre: Z) (suffix_2: (@list Z)) (out: Z) (bits: Z) (x: Z) (num: Z) (PreH1 : (num > 0)) (PreH2 : (0 <= num)) (PreH3 : (num <= num_pre)) (PreH4 : (0 < num_pre)) (PreH5 : (num_pre <= INT_MAX)) (PreH6 : (x = 0)) (PreH7 : (0 <= bits)) (PreH8 : (bits <= (binary_length_z_103 (num_pre)))) (PreH9 : (out <> 0)) (PreH10 : (binary_safe_103 num_pre )) (PreH11 : (binary_backfill_state_z_103 num_pre num bits suffix_2 )) (PreH12 : ((Zlength (suffix_2)) = (((binary_length_z_103 (num_pre)) + 1 ) - bits ))) ,
+  (CharArray.undef_seg out 0 bits )
+|--
+  (CharArray.undef_full out bits )
+.
+
+Definition to_binary_string_entail_wit_7 := 
+(
+forall (num_pre: Z) (suffix_2: (@list Z)) (num: Z) (x: Z) (bits: Z) (out: Z) (PreH1 : (0 < num)) (PreH2 : (num <= num_pre)) (PreH3 : (0 < num_pre)) (PreH4 : (num_pre <= INT_MAX)) (PreH5 : (x = 0)) (PreH6 : (0 < bits)) (PreH7 : (bits <= (binary_length_z_103 (num_pre)))) (PreH8 : (out <> 0)) (PreH9 : (binary_safe_103 num_pre )) (PreH10 : (binary_backfill_state_z_103 num_pre num bits suffix_2 )) (PreH11 : ((Zlength (suffix_2)) = (((binary_length_z_103 (num_pre)) + 1 ) - bits ))) ,
+  (((out + ((bits - 1 ) * sizeof(CHAR) ) )) # Char  |-> (signed_last_nbits ((48 + (num % ( 2 ) ) )) (8)))
+  **  (CharArray.undef_missing_i out (bits - 1 ) 0 bits )
+  **  (CharArray.seg out bits ((binary_length_z_103 (num_pre)) + 1 ) suffix_2 )
+|--
+  EX (suffix: (@list Z)) ,
+  “ (0 < num) ” 
+  &&  “ (num <= num_pre) ” 
+  &&  “ (0 < num_pre) ” 
+  &&  “ (num_pre <= INT_MAX) ” 
+  &&  “ (x = 0) ” 
+  &&  “ (0 < bits) ” 
+  &&  “ (bits <= (binary_length_z_103 (num_pre))) ” 
+  &&  “ (out <> 0) ” 
+  &&  “ (binary_safe_103 num_pre ) ” 
+  &&  “ (binary_backfill_state_z_103 num_pre (num ÷ 2 ) (bits - 1 ) (cons ((48 + (num % ( 2 ) ) )) (suffix)) ) ” 
+  &&  “ ((Zlength ((cons ((48 + (num % ( 2 ) ) )) (suffix)))) = (((binary_length_z_103 (num_pre)) + 1 ) - (bits - 1 ) )) ”
+  &&  (CharArray.undef_seg out 0 (bits - 1 ) )
+  **  (CharArray.seg out (bits - 1 ) ((binary_length_z_103 (num_pre)) + 1 ) (cons ((48 + (num % ( 2 ) ) )) (suffix)) )
+) \/
+(
+forall (num_pre: Z) (suffix_2: (@list Z)) (num: Z) (x: Z) (bits: Z) (out: Z) (PreH1 : (0 < num)) (PreH2 : (num <= num_pre)) (PreH3 : (0 < num_pre)) (PreH4 : (num_pre <= INT_MAX)) (PreH5 : (x = 0)) (PreH6 : (0 < bits)) (PreH7 : (bits <= (binary_length_z_103 (num_pre)))) (PreH8 : (out <> 0)) (PreH9 : (binary_safe_103 num_pre )) (PreH10 : (binary_backfill_state_z_103 num_pre num bits suffix_2 )) (PreH11 : ((Zlength (suffix_2)) = (((binary_length_z_103 (num_pre)) + 1 ) - bits ))) ,
+  (((out + ((bits - 1 ) * sizeof(CHAR) ) )) # Char  |-> (signed_last_nbits ((48 + (num % ( 2 ) ) )) (8)))
+  **  (CharArray.undef_missing_i out (bits - 1 ) 0 bits )
+  **  (CharArray.seg out bits ((binary_length_z_103 (num_pre)) + 1 ) suffix_2 )
+|--
+  EX (suffix: (@list Z)) ,
+  “ (0 < num) ” 
+  &&  “ (num <= num_pre) ” 
+  &&  “ (0 < num_pre) ” 
+  &&  “ (num_pre <= INT_MAX) ” 
+  &&  “ (x = 0) ” 
+  &&  “ (0 < bits) ” 
+  &&  “ (bits <= (binary_length_z_103 (num_pre))) ” 
+  &&  “ (out <> 0) ” 
+  &&  “ (binary_safe_103 num_pre ) ” 
+  &&  “ (binary_backfill_state_z_103 num_pre (num ÷ 2 ) (bits - 1 ) (cons ((48 + (num % ( 2 ) ) )) (suffix)) ) ” 
+  &&  “ ((Zlength ((cons ((48 + (num % ( 2 ) ) )) (suffix)))) = (((binary_length_z_103 (num_pre)) + 1 ) - (bits - 1 ) )) ”
+  &&  (CharArray.undef_full out (bits - 1 ) )
+  **  (CharArray.seg out (bits - 1 ) ((binary_length_z_103 (num_pre)) + 1 ) (cons ((48 + (num % ( 2 ) ) )) (suffix)) )
+).
+
+Definition to_binary_string_entail_wit_8 := 
+(
+forall (num_pre: Z) (suffix_2: (@list Z)) (num: Z) (x: Z) (bits: Z) (out: Z) (PreH1 : (0 < num)) (PreH2 : (num <= num_pre)) (PreH3 : (0 < num_pre)) (PreH4 : (num_pre <= INT_MAX)) (PreH5 : (x = 0)) (PreH6 : (0 < bits)) (PreH7 : (bits <= (binary_length_z_103 (num_pre)))) (PreH8 : (out <> 0)) (PreH9 : (binary_safe_103 num_pre )) (PreH10 : (binary_backfill_state_z_103 num_pre (num ÷ 2 ) (bits - 1 ) (cons ((48 + (num % ( 2 ) ) )) (suffix_2)) )) (PreH11 : ((Zlength ((cons ((48 + (num % ( 2 ) ) )) (suffix_2)))) = (((binary_length_z_103 (num_pre)) + 1 ) - (bits - 1 ) ))) ,
+  (CharArray.undef_seg out 0 (bits - 1 ) )
+  **  (CharArray.seg out (bits - 1 ) ((binary_length_z_103 (num_pre)) + 1 ) (cons ((48 + (num % ( 2 ) ) )) (suffix_2)) )
+|--
+  EX (suffix: (@list Z)) ,
+  “ (0 <= (num ÷ 2 )) ” 
+  &&  “ ((num ÷ 2 ) <= num_pre) ” 
+  &&  “ (0 < num_pre) ” 
+  &&  “ (num_pre <= INT_MAX) ” 
+  &&  “ (x = 0) ” 
+  &&  “ (0 <= (bits - 1 )) ” 
+  &&  “ ((bits - 1 ) <= (binary_length_z_103 (num_pre))) ” 
+  &&  “ (out <> 0) ” 
+  &&  “ (binary_safe_103 num_pre ) ” 
+  &&  “ (binary_backfill_state_z_103 num_pre (num ÷ 2 ) (bits - 1 ) suffix ) ” 
+  &&  “ ((Zlength (suffix)) = (((binary_length_z_103 (num_pre)) + 1 ) - (bits - 1 ) )) ”
+  &&  (CharArray.undef_seg out 0 (bits - 1 ) )
+  **  (CharArray.seg out (bits - 1 ) ((binary_length_z_103 (num_pre)) + 1 ) suffix )
+) \/
+(
+forall (num_pre: Z) (suffix_2: (@list Z)) (num: Z) (x: Z) (bits: Z) (out: Z) (PreH1 : (0 < num)) (PreH2 : (num <= num_pre)) (PreH3 : (0 < num_pre)) (PreH4 : (num_pre <= INT_MAX)) (PreH5 : (x = 0)) (PreH6 : (0 < bits)) (PreH7 : (bits <= (binary_length_z_103 (num_pre)))) (PreH8 : (out <> 0)) (PreH9 : (binary_safe_103 num_pre )) (PreH10 : (binary_backfill_state_z_103 num_pre (num ÷ 2 ) (bits - 1 ) (cons ((48 + (num % ( 2 ) ) )) (suffix_2)) )) (PreH11 : ((Zlength ((cons ((48 + (num % ( 2 ) ) )) (suffix_2)))) = (((binary_length_z_103 (num_pre)) + 1 ) - (bits - 1 ) ))) ,
+  (CharArray.undef_seg out 0 (bits - 1 ) )
+|--
+  “ ((num ÷ 2 ) <= num_pre) ” 
+  &&  “ (0 <= (num ÷ 2 )) ”
+  &&  (CharArray.undef_full out (bits - 1 ) )
+).
+
+Definition to_binary_string_entail_wit_8_split_goal_1 := 
+forall (num_pre: Z) (suffix_2: (@list Z)) (num: Z) (x: Z) (bits: Z) (out: Z) (PreH1 : (0 < num)) (PreH2 : (num <= num_pre)) (PreH3 : (0 < num_pre)) (PreH4 : (num_pre <= INT_MAX)) (PreH5 : (x = 0)) (PreH6 : (0 < bits)) (PreH7 : (bits <= (binary_length_z_103 (num_pre)))) (PreH8 : (out <> 0)) (PreH9 : (binary_safe_103 num_pre )) (PreH10 : (binary_backfill_state_z_103 num_pre (num ÷ 2 ) (bits - 1 ) (cons ((48 + (num % ( 2 ) ) )) (suffix_2)) )) (PreH11 : ((Zlength ((cons ((48 + (num % ( 2 ) ) )) (suffix_2)))) = (((binary_length_z_103 (num_pre)) + 1 ) - (bits - 1 ) ))) ,
+  (CharArray.undef_seg out 0 (bits - 1 ) )
+|--
+  “ ((num ÷ 2 ) <= num_pre) ”
+.
+
+Definition to_binary_string_entail_wit_8_split_goal_2 := 
+forall (num_pre: Z) (suffix_2: (@list Z)) (num: Z) (x: Z) (bits: Z) (out: Z) (PreH1 : (0 < num)) (PreH2 : (num <= num_pre)) (PreH3 : (0 < num_pre)) (PreH4 : (num_pre <= INT_MAX)) (PreH5 : (x = 0)) (PreH6 : (0 < bits)) (PreH7 : (bits <= (binary_length_z_103 (num_pre)))) (PreH8 : (out <> 0)) (PreH9 : (binary_safe_103 num_pre )) (PreH10 : (binary_backfill_state_z_103 num_pre (num ÷ 2 ) (bits - 1 ) (cons ((48 + (num % ( 2 ) ) )) (suffix_2)) )) (PreH11 : ((Zlength ((cons ((48 + (num % ( 2 ) ) )) (suffix_2)))) = (((binary_length_z_103 (num_pre)) + 1 ) - (bits - 1 ) ))) ,
+  (CharArray.undef_seg out 0 (bits - 1 ) )
+|--
+  “ (0 <= (num ÷ 2 )) ”
+.
+
+Definition to_binary_string_entail_wit_8_split_goal_spatial := 
+forall (num_pre: Z) (suffix_2: (@list Z)) (num: Z) (x: Z) (bits: Z) (out: Z) (PreH1 : (0 < num)) (PreH2 : (num <= num_pre)) (PreH3 : (0 < num_pre)) (PreH4 : (num_pre <= INT_MAX)) (PreH5 : (x = 0)) (PreH6 : (0 < bits)) (PreH7 : (bits <= (binary_length_z_103 (num_pre)))) (PreH8 : (out <> 0)) (PreH9 : (binary_safe_103 num_pre )) (PreH10 : (binary_backfill_state_z_103 num_pre (num ÷ 2 ) (bits - 1 ) (cons ((48 + (num % ( 2 ) ) )) (suffix_2)) )) (PreH11 : ((Zlength ((cons ((48 + (num % ( 2 ) ) )) (suffix_2)))) = (((binary_length_z_103 (num_pre)) + 1 ) - (bits - 1 ) ))) ,
+  (CharArray.undef_seg out 0 (bits - 1 ) )
+|--
+  (CharArray.undef_full out (bits - 1 ) )
+.
+
+Definition to_binary_string_entail_wit_9 := 
+(
+forall (num_pre: Z) (suffix_2: (@list Z)) (out: Z) (bits: Z) (x: Z) (num: Z) (PreH1 : (num <= 0)) (PreH2 : (0 <= num)) (PreH3 : (num <= num_pre)) (PreH4 : (0 < num_pre)) (PreH5 : (num_pre <= INT_MAX)) (PreH6 : (x = 0)) (PreH7 : (0 <= bits)) (PreH8 : (bits <= (binary_length_z_103 (num_pre)))) (PreH9 : (out <> 0)) (PreH10 : (binary_safe_103 num_pre )) (PreH11 : (binary_backfill_state_z_103 num_pre num bits suffix_2 )) (PreH12 : ((Zlength (suffix_2)) = (((binary_length_z_103 (num_pre)) + 1 ) - bits ))) ,
+  (CharArray.undef_seg out 0 bits )
+  **  (CharArray.seg out bits ((binary_length_z_103 (num_pre)) + 1 ) suffix_2 )
+|--
+  EX (suffix: (@list Z)) ,
+  “ (num = 0) ” 
+  &&  “ (0 < num_pre) ” 
+  &&  “ (num_pre <= INT_MAX) ” 
+  &&  “ (x = 0) ” 
+  &&  “ (bits = 0) ” 
+  &&  “ (out <> 0) ” 
+  &&  “ (binary_safe_103 num_pre ) ” 
+  &&  “ (suffix = (app ((binary_output_z_103 (num_pre))) ((cons (0) ((@nil Z)))))) ” 
+  &&  “ ((Zlength (suffix)) = ((binary_length_z_103 (num_pre)) + 1 )) ”
+  &&  (CharArray.seg out 0 ((binary_length_z_103 (num_pre)) + 1 ) suffix )
+) \/
+(
+forall (num_pre: Z) (suffix_2: (@list Z)) (out: Z) (bits: Z) (x: Z) (num: Z) (PreH1 : (num <= 0)) (PreH2 : (0 <= num)) (PreH3 : (num <= num_pre)) (PreH4 : (0 < num_pre)) (PreH5 : (num_pre <= INT_MAX)) (PreH6 : (x = 0)) (PreH7 : (0 <= bits)) (PreH8 : (bits <= (binary_length_z_103 (num_pre)))) (PreH9 : (out <> 0)) (PreH10 : (binary_safe_103 num_pre )) (PreH11 : (binary_backfill_state_z_103 num_pre num bits suffix_2 )) (PreH12 : ((Zlength (suffix_2)) = (((binary_length_z_103 (num_pre)) + 1 ) - bits ))) ,
+  (CharArray.undef_seg out 0 bits )
+  **  (CharArray.seg out bits ((binary_length_z_103 (num_pre)) + 1 ) suffix_2 )
+|--
+  “ ((Zlength ((app ((binary_output_z_103 (num_pre))) ((cons (0) ((@nil Z))))))) = ((binary_length_z_103 (num_pre)) + 1 )) ” 
+  &&  “ (bits = 0) ”
+  &&  (CharArray.seg out 0 ((binary_length_z_103 (num_pre)) + 1 ) (app ((binary_output_z_103 (num_pre))) ((cons (0) ((@nil Z))))) )
+).
+
+Definition to_binary_string_entail_wit_9_split_goal_1 := 
+forall (num_pre: Z) (suffix_2: (@list Z)) (out: Z) (bits: Z) (x: Z) (num: Z) (PreH1 : (num <= 0)) (PreH2 : (0 <= num)) (PreH3 : (num <= num_pre)) (PreH4 : (0 < num_pre)) (PreH5 : (num_pre <= INT_MAX)) (PreH6 : (x = 0)) (PreH7 : (0 <= bits)) (PreH8 : (bits <= (binary_length_z_103 (num_pre)))) (PreH9 : (out <> 0)) (PreH10 : (binary_safe_103 num_pre )) (PreH11 : (binary_backfill_state_z_103 num_pre num bits suffix_2 )) (PreH12 : ((Zlength (suffix_2)) = (((binary_length_z_103 (num_pre)) + 1 ) - bits ))) ,
+  (CharArray.undef_seg out 0 bits )
+  **  (CharArray.seg out bits ((binary_length_z_103 (num_pre)) + 1 ) suffix_2 )
+|--
+  “ ((Zlength ((app ((binary_output_z_103 (num_pre))) ((cons (0) ((@nil Z))))))) = ((binary_length_z_103 (num_pre)) + 1 )) ”
+.
+
+Definition to_binary_string_entail_wit_9_split_goal_2 := 
+forall (num_pre: Z) (suffix_2: (@list Z)) (out: Z) (bits: Z) (x: Z) (num: Z) (PreH1 : (num <= 0)) (PreH2 : (0 <= num)) (PreH3 : (num <= num_pre)) (PreH4 : (0 < num_pre)) (PreH5 : (num_pre <= INT_MAX)) (PreH6 : (x = 0)) (PreH7 : (0 <= bits)) (PreH8 : (bits <= (binary_length_z_103 (num_pre)))) (PreH9 : (out <> 0)) (PreH10 : (binary_safe_103 num_pre )) (PreH11 : (binary_backfill_state_z_103 num_pre num bits suffix_2 )) (PreH12 : ((Zlength (suffix_2)) = (((binary_length_z_103 (num_pre)) + 1 ) - bits ))) ,
+  (CharArray.undef_seg out 0 bits )
+  **  (CharArray.seg out bits ((binary_length_z_103 (num_pre)) + 1 ) suffix_2 )
+|--
+  “ (bits = 0) ”
+.
+
+Definition to_binary_string_entail_wit_9_split_goal_spatial := 
+forall (num_pre: Z) (suffix_2: (@list Z)) (out: Z) (bits: Z) (x: Z) (num: Z) (PreH1 : (num <= 0)) (PreH2 : (0 <= num)) (PreH3 : (num <= num_pre)) (PreH4 : (0 < num_pre)) (PreH5 : (num_pre <= INT_MAX)) (PreH6 : (x = 0)) (PreH7 : (0 <= bits)) (PreH8 : (bits <= (binary_length_z_103 (num_pre)))) (PreH9 : (out <> 0)) (PreH10 : (binary_safe_103 num_pre )) (PreH11 : (binary_backfill_state_z_103 num_pre num bits suffix_2 )) (PreH12 : ((Zlength (suffix_2)) = (((binary_length_z_103 (num_pre)) + 1 ) - bits ))) ,
+  (CharArray.undef_seg out 0 bits )
+  **  (CharArray.seg out bits ((binary_length_z_103 (num_pre)) + 1 ) suffix_2 )
+|--
+  (CharArray.seg out 0 ((binary_length_z_103 (num_pre)) + 1 ) (app ((binary_output_z_103 (num_pre))) ((cons (0) ((@nil Z))))) )
+.
+
+Definition to_binary_string_return_wit_1 := 
+(
+forall (num_pre: Z) (suffix: (@list Z)) (num: Z) (x: Z) (bits: Z) (out: Z) (PreH1 : (num = 0)) (PreH2 : (0 < num_pre)) (PreH3 : (num_pre <= INT_MAX)) (PreH4 : (x = 0)) (PreH5 : (bits = 0)) (PreH6 : (out <> 0)) (PreH7 : (binary_safe_103 num_pre )) (PreH8 : (suffix = (app ((binary_output_z_103 (num_pre))) ((cons (0) ((@nil Z))))))) (PreH9 : ((Zlength (suffix)) = ((binary_length_z_103 (num_pre)) + 1 ))) ,
+  (CharArray.seg out 0 ((binary_length_z_103 (num_pre)) + 1 ) suffix )
+|--
+  EX (out_l: (@list Z))  (len: Z) ,
+  “ (len = (Zlength (out_l))) ” 
+  &&  “ (len = (binary_length_z_103 (num_pre))) ” 
+  &&  “ (out_l = (binary_output_z_103 (num_pre))) ”
+  &&  (CharArray.full out (len + 1 ) (app (out_l) ((cons (0) ((@nil Z))))) )
+) \/
+(
+forall (num_pre: Z) (suffix: (@list Z)) (num: Z) (x: Z) (bits: Z) (out: Z) (PreH1 : (num = 0)) (PreH2 : (0 < num_pre)) (PreH3 : (num_pre <= INT_MAX)) (PreH4 : (x = 0)) (PreH5 : (bits = 0)) (PreH6 : (out <> 0)) (PreH7 : (binary_safe_103 num_pre )) (PreH8 : (suffix = (app ((binary_output_z_103 (num_pre))) ((cons (0) ((@nil Z))))))) (PreH9 : ((Zlength (suffix)) = ((binary_length_z_103 (num_pre)) + 1 ))) ,
+  (CharArray.seg out 0 ((binary_length_z_103 (num_pre)) + 1 ) suffix )
+|--
+  “ ((Zlength ((binary_output_z_103 (num_pre)))) = (binary_length_z_103 (num_pre))) ”
+  &&  (CharArray.full out ((Zlength ((binary_output_z_103 (num_pre)))) + 1 ) (app ((binary_output_z_103 (num_pre))) ((cons (0) ((@nil Z))))) )
+).
+
+Definition to_binary_string_return_wit_1_split_goal_1 := 
+forall (num_pre: Z) (suffix: (@list Z)) (num: Z) (x: Z) (bits: Z) (out: Z) (PreH1 : (num = 0)) (PreH2 : (0 < num_pre)) (PreH3 : (num_pre <= INT_MAX)) (PreH4 : (x = 0)) (PreH5 : (bits = 0)) (PreH6 : (out <> 0)) (PreH7 : (binary_safe_103 num_pre )) (PreH8 : (suffix = (app ((binary_output_z_103 (num_pre))) ((cons (0) ((@nil Z))))))) (PreH9 : ((Zlength (suffix)) = ((binary_length_z_103 (num_pre)) + 1 ))) ,
+  (CharArray.seg out 0 ((binary_length_z_103 (num_pre)) + 1 ) suffix )
+|--
+  “ ((Zlength ((binary_output_z_103 (num_pre)))) = (binary_length_z_103 (num_pre))) ”
+.
+
+Definition to_binary_string_return_wit_1_split_goal_spatial := 
+forall (num_pre: Z) (suffix: (@list Z)) (num: Z) (x: Z) (bits: Z) (out: Z) (PreH1 : (num = 0)) (PreH2 : (0 < num_pre)) (PreH3 : (num_pre <= INT_MAX)) (PreH4 : (x = 0)) (PreH5 : (bits = 0)) (PreH6 : (out <> 0)) (PreH7 : (binary_safe_103 num_pre )) (PreH8 : (suffix = (app ((binary_output_z_103 (num_pre))) ((cons (0) ((@nil Z))))))) (PreH9 : ((Zlength (suffix)) = ((binary_length_z_103 (num_pre)) + 1 ))) ,
+  (CharArray.seg out 0 ((binary_length_z_103 (num_pre)) + 1 ) suffix )
+|--
+  (CharArray.full out ((Zlength ((binary_output_z_103 (num_pre)))) + 1 ) (app ((binary_output_z_103 (num_pre))) ((cons (0) ((@nil Z))))) )
+.
+
+Definition to_binary_string_return_wit_2 := 
+(
+forall (num_pre: Z) (retval: Z) (PreH1 : (retval <> 0)) (PreH2 : (num_pre = 0)) (PreH3 : (0 <= num_pre)) (PreH4 : (num_pre <= INT_MAX)) (PreH5 : (binary_safe_103 num_pre )) ,
+  (CharArray.undef_seg retval (1 + 1 ) 2 )
+  **  (((retval + (1 * sizeof(CHAR) ) )) # Char  |-> 0)
+  **  (((retval + (0 * sizeof(CHAR) ) )) # Char  |-> 48)
+|--
+  EX (out_l: (@list Z))  (len: Z) ,
+  “ (len = (Zlength (out_l))) ” 
+  &&  “ (len = (binary_length_z_103 (num_pre))) ” 
+  &&  “ (out_l = (binary_output_z_103 (num_pre))) ”
+  &&  (CharArray.full retval (len + 1 ) (app (out_l) ((cons (0) ((@nil Z))))) )
+) \/
+(
+forall (num_pre: Z) (retval: Z) (PreH1 : (retval <> 0)) (PreH2 : (num_pre = 0)) (PreH3 : (0 <= num_pre)) (PreH4 : (num_pre <= INT_MAX)) (PreH5 : (binary_safe_103 num_pre )) ,
+  (((retval + (1 * sizeof(CHAR) ) )) # Char  |-> 0)
+  **  (((retval + (0 * sizeof(CHAR) ) )) # Char  |-> 48)
+|--
+  “ ((Zlength ((binary_output_z_103 (num_pre)))) = (binary_length_z_103 (num_pre))) ”
+  &&  (CharArray.full retval ((Zlength ((binary_output_z_103 (num_pre)))) + 1 ) (app ((binary_output_z_103 (num_pre))) ((cons (0) ((@nil Z))))) )
+).
+
+Definition to_binary_string_return_wit_2_split_goal_1 := 
+forall (num_pre: Z) (retval: Z) (PreH1 : (retval <> 0)) (PreH2 : (num_pre = 0)) (PreH3 : (0 <= num_pre)) (PreH4 : (num_pre <= INT_MAX)) (PreH5 : (binary_safe_103 num_pre )) ,
+  (((retval + (1 * sizeof(CHAR) ) )) # Char  |-> 0)
+  **  (((retval + (0 * sizeof(CHAR) ) )) # Char  |-> 48)
+|--
+  “ ((Zlength ((binary_output_z_103 (num_pre)))) = (binary_length_z_103 (num_pre))) ”
+.
+
+Definition to_binary_string_return_wit_2_split_goal_spatial := 
+forall (num_pre: Z) (retval: Z) (PreH1 : (retval <> 0)) (PreH2 : (num_pre = 0)) (PreH3 : (0 <= num_pre)) (PreH4 : (num_pre <= INT_MAX)) (PreH5 : (binary_safe_103 num_pre )) ,
+  (((retval + (1 * sizeof(CHAR) ) )) # Char  |-> 0)
+  **  (((retval + (0 * sizeof(CHAR) ) )) # Char  |-> 48)
+|--
+  (CharArray.full retval ((Zlength ((binary_output_z_103 (num_pre)))) + 1 ) (app ((binary_output_z_103 (num_pre))) ((cons (0) ((@nil Z))))) )
+.
+
+Definition to_binary_string_partial_solve_wit_1_pure := 
+forall (num_pre: Z) (PreH1 : (num_pre = 0)) (PreH2 : (0 <= num_pre)) (PreH3 : (num_pre <= INT_MAX)) (PreH4 : (binary_safe_103 num_pre )) ,
+  ((( &( "out" ) )) # Ptr  |-> 0)
+  **  ((( &( "x" ) )) # Int  |-> num_pre)
+  **  ((( &( "bits" ) )) # Int  |-> 0)
+  **  ((( &( "num" ) )) # Int  |-> num_pre)
+|--
+  “ (2 > 0) ” 
+  &&  “ (2 < INT_MAX) ”
+.
+
+Definition to_binary_string_partial_solve_wit_1_aux := 
+forall (num_pre: Z) (PreH1 : (num_pre = 0)) (PreH2 : (0 <= num_pre)) (PreH3 : (num_pre <= INT_MAX)) (PreH4 : (binary_safe_103 num_pre )) ,
+  TT && emp 
+|--
+  “ (2 > 0) ” 
+  &&  “ (2 < INT_MAX) ” 
+  &&  “ (num_pre = 0) ” 
+  &&  “ (0 <= num_pre) ” 
+  &&  “ (num_pre <= INT_MAX) ” 
+  &&  “ (binary_safe_103 num_pre ) ”
+  &&  emp
+.
+
+Definition to_binary_string_partial_solve_wit_1 := to_binary_string_partial_solve_wit_1_pure -> to_binary_string_partial_solve_wit_1_aux.
+
+Definition to_binary_string_partial_solve_wit_2 := 
+forall (num_pre: Z) (retval: Z) (PreH1 : (retval <> 0)) (PreH2 : (num_pre = 0)) (PreH3 : (0 <= num_pre)) (PreH4 : (num_pre <= INT_MAX)) (PreH5 : (binary_safe_103 num_pre )) ,
+  (CharArray.undef_full retval 2 )
+|--
+  “ (retval <> 0) ” 
+  &&  “ (num_pre = 0) ” 
+  &&  “ (0 <= num_pre) ” 
+  &&  “ (num_pre <= INT_MAX) ” 
+  &&  “ (binary_safe_103 num_pre ) ”
+  &&  (((retval + (0 * sizeof(CHAR) ) )) # Char  |->_)
+  **  (CharArray.undef_missing_i retval 0 0 2 )
+.
+
+Definition to_binary_string_partial_solve_wit_3 := 
+forall (num_pre: Z) (retval: Z) (PreH1 : (retval <> 0)) (PreH2 : (num_pre = 0)) (PreH3 : (0 <= num_pre)) (PreH4 : (num_pre <= INT_MAX)) (PreH5 : (binary_safe_103 num_pre )) ,
+  (CharArray.undef_seg retval (0 + 1 ) 2 )
+  **  (((retval + (0 * sizeof(CHAR) ) )) # Char  |-> 48)
+|--
+  “ (retval <> 0) ” 
+  &&  “ (num_pre = 0) ” 
+  &&  “ (0 <= num_pre) ” 
+  &&  “ (num_pre <= INT_MAX) ” 
+  &&  “ (binary_safe_103 num_pre ) ”
+  &&  (((retval + (1 * sizeof(CHAR) ) )) # Char  |->_)
+  **  (CharArray.undef_missing_i retval 1 (0 + 1 ) 2 )
+  **  (((retval + (0 * sizeof(CHAR) ) )) # Char  |-> 48)
+.
+
+Definition to_binary_string_partial_solve_wit_4_pure := 
+(
+forall (num_pre: Z) (x: Z) (bits: Z) (out: Z) (PreH1 : (0 < num_pre)) (PreH2 : (num_pre <= INT_MAX)) (PreH3 : (x = 0)) (PreH4 : (bits = (binary_length_z_103 (num_pre)))) (PreH5 : (1 <= bits)) (PreH6 : (out = 0)) (PreH7 : (binary_safe_103 num_pre )) ,
+  ((( &( "num" ) )) # Int  |-> num_pre)
+  **  ((( &( "x" ) )) # Int  |-> x)
+  **  ((( &( "bits" ) )) # Int  |-> bits)
+  **  ((( &( "out" ) )) # Ptr  |-> out)
+|--
+  “ ((bits + 1 ) > 0) ” 
+  &&  “ ((bits + 1 ) < INT_MAX) ”
+) \/
+(
+forall (num_pre: Z) (x: Z) (bits: Z) (out: Z) (PreH1 : (bits <= INT_MAX)) (PreH2 : (x <= INT_MAX)) (PreH3 : (bits >= INT_MIN)) (PreH4 : (x >= INT_MIN)) (PreH5 : (num_pre >= INT_MIN)) (PreH6 : (0 < num_pre)) (PreH7 : (num_pre <= INT_MAX)) (PreH8 : (x = 0)) (PreH9 : (bits = (binary_length_z_103 (num_pre)))) (PreH10 : (1 <= bits)) (PreH11 : (out = 0)) (PreH12 : (binary_safe_103 num_pre )) ,
+  ((( &( "num" ) )) # Int  |-> num_pre)
+  **  ((( &( "x" ) )) # Int  |-> x)
+  **  ((( &( "bits" ) )) # Int  |-> bits)
+  **  ((( &( "out" ) )) # Ptr  |-> out)
+|--
+  “ ((bits + 1 ) < INT_MAX) ”
+).
+
+Definition to_binary_string_partial_solve_wit_4_pure_split_goal_1 := 
+forall (num_pre: Z) (x: Z) (bits: Z) (out: Z) (PreH1 : (bits <= INT_MAX)) (PreH2 : (x <= INT_MAX)) (PreH3 : (bits >= INT_MIN)) (PreH4 : (x >= INT_MIN)) (PreH5 : (num_pre >= INT_MIN)) (PreH6 : (0 < num_pre)) (PreH7 : (num_pre <= INT_MAX)) (PreH8 : (x = 0)) (PreH9 : (bits = (binary_length_z_103 (num_pre)))) (PreH10 : (1 <= bits)) (PreH11 : (out = 0)) (PreH12 : (binary_safe_103 num_pre )) ,
+  ((( &( "num" ) )) # Int  |-> num_pre)
+  **  ((( &( "x" ) )) # Int  |-> x)
+  **  ((( &( "bits" ) )) # Int  |-> bits)
+  **  ((( &( "out" ) )) # Ptr  |-> out)
+|--
+  “ ((bits + 1 ) < INT_MAX) ”
+.
+
+Definition to_binary_string_partial_solve_wit_4_aux := 
+forall (num_pre: Z) (x: Z) (bits: Z) (out: Z) (PreH1 : (0 < num_pre)) (PreH2 : (num_pre <= INT_MAX)) (PreH3 : (x = 0)) (PreH4 : (bits = (binary_length_z_103 (num_pre)))) (PreH5 : (1 <= bits)) (PreH6 : (out = 0)) (PreH7 : (binary_safe_103 num_pre )) ,
+  TT && emp 
+|--
+  “ ((bits + 1 ) > 0) ” 
+  &&  “ ((bits + 1 ) < INT_MAX) ” 
+  &&  “ (0 < num_pre) ” 
+  &&  “ (num_pre <= INT_MAX) ” 
+  &&  “ (x = 0) ” 
+  &&  “ (bits = (binary_length_z_103 (num_pre))) ” 
+  &&  “ (1 <= bits) ” 
+  &&  “ (out = 0) ” 
+  &&  “ (binary_safe_103 num_pre ) ”
+  &&  emp
+.
+
+Definition to_binary_string_partial_solve_wit_4 := to_binary_string_partial_solve_wit_4_pure -> to_binary_string_partial_solve_wit_4_aux.
+
+Definition to_binary_string_partial_solve_wit_5 := 
+forall (num_pre: Z) (x: Z) (bits: Z) (out: Z) (retval: Z) (PreH1 : (retval <> 0)) (PreH2 : (0 < num_pre)) (PreH3 : (num_pre <= INT_MAX)) (PreH4 : (x = 0)) (PreH5 : (bits = (binary_length_z_103 (num_pre)))) (PreH6 : (1 <= bits)) (PreH7 : (out = 0)) (PreH8 : (binary_safe_103 num_pre )) ,
+  (CharArray.undef_full retval (bits + 1 ) )
+|--
+  “ (retval <> 0) ” 
+  &&  “ (0 < num_pre) ” 
+  &&  “ (num_pre <= INT_MAX) ” 
+  &&  “ (x = 0) ” 
+  &&  “ (bits = (binary_length_z_103 (num_pre))) ” 
+  &&  “ (1 <= bits) ” 
+  &&  “ (out = 0) ” 
+  &&  “ (binary_safe_103 num_pre ) ”
+  &&  (((retval + (bits * sizeof(CHAR) ) )) # Char  |->_)
+  **  (CharArray.undef_missing_i retval bits 0 (bits + 1 ) )
+.
+
+Definition to_binary_string_partial_solve_wit_6 := 
+forall (num_pre: Z) (suffix: (@list Z)) (num: Z) (x: Z) (bits: Z) (out: Z) (PreH1 : (0 < num)) (PreH2 : (num <= num_pre)) (PreH3 : (0 < num_pre)) (PreH4 : (num_pre <= INT_MAX)) (PreH5 : (x = 0)) (PreH6 : (0 < bits)) (PreH7 : (bits <= (binary_length_z_103 (num_pre)))) (PreH8 : (out <> 0)) (PreH9 : (binary_safe_103 num_pre )) (PreH10 : (binary_backfill_state_z_103 num_pre num bits suffix )) (PreH11 : ((Zlength (suffix)) = (((binary_length_z_103 (num_pre)) + 1 ) - bits ))) ,
+  (CharArray.undef_seg out 0 bits )
+  **  (CharArray.seg out bits ((binary_length_z_103 (num_pre)) + 1 ) suffix )
+|--
+  “ (0 < num) ” 
+  &&  “ (num <= num_pre) ” 
+  &&  “ (0 < num_pre) ” 
+  &&  “ (num_pre <= INT_MAX) ” 
+  &&  “ (x = 0) ” 
+  &&  “ (0 < bits) ” 
+  &&  “ (bits <= (binary_length_z_103 (num_pre))) ” 
+  &&  “ (out <> 0) ” 
+  &&  “ (binary_safe_103 num_pre ) ” 
+  &&  “ (binary_backfill_state_z_103 num_pre num bits suffix ) ” 
+  &&  “ ((Zlength (suffix)) = (((binary_length_z_103 (num_pre)) + 1 ) - bits )) ”
+  &&  (((out + ((bits - 1 ) * sizeof(CHAR) ) )) # Char  |->_)
+  **  (CharArray.undef_missing_i out (bits - 1 ) 0 bits )
+  **  (CharArray.seg out bits ((binary_length_z_103 (num_pre)) + 1 ) suffix )
+.
+
+(*----- Function rounded_avg -----*)
+
+Definition rounded_avg_safety_wit_1 := 
+forall (m_pre: Z) (n_pre: Z) (PreH1 : (n_pre > m_pre)) (PreH2 : (0 < n_pre)) (PreH3 : (n_pre <= INT_MAX)) (PreH4 : (0 < m_pre)) (PreH5 : (m_pre <= INT_MAX)) (PreH6 : ((n_pre + m_pre ) <= INT_MAX)) (PreH7 : (problem_103_pre_z n_pre m_pre )) (PreH8 : (rounded_avg_safe_103 n_pre m_pre )) ,
+  ((( &( "out" ) )) # Ptr  |->_)
+  **  ((( &( "num" ) )) # Int  |->_)
+  **  ((( &( "m" ) )) # Int  |-> m_pre)
+  **  ((( &( "n" ) )) # Int  |-> n_pre)
+|--
+  “ (3 <= INT_MAX) ” 
+  &&  “ ((INT_MIN) <= 3) ”
+.
+
+Definition rounded_avg_safety_wit_2 := 
+forall (m_pre: Z) (n_pre: Z) (retval: Z) (PreH1 : (retval <> 0)) (PreH2 : (n_pre > m_pre)) (PreH3 : (0 < n_pre)) (PreH4 : (n_pre <= INT_MAX)) (PreH5 : (0 < m_pre)) (PreH6 : (m_pre <= INT_MAX)) (PreH7 : ((n_pre + m_pre ) <= INT_MAX)) (PreH8 : (problem_103_pre_z n_pre m_pre )) (PreH9 : (rounded_avg_safe_103 n_pre m_pre )) ,
+  (CharArray.undef_full retval 3 )
+  **  ((( &( "out" ) )) # Ptr  |-> retval)
+  **  ((( &( "num" ) )) # Int  |->_)
+  **  ((( &( "m" ) )) # Int  |-> m_pre)
+  **  ((( &( "n" ) )) # Int  |-> n_pre)
+|--
+  “ (0 <= INT_MAX) ” 
+  &&  “ ((INT_MIN) <= 0) ”
+.
+
+Definition rounded_avg_safety_wit_3 := 
+forall (m_pre: Z) (n_pre: Z) (retval: Z) (PreH1 : (retval <> 0)) (PreH2 : (n_pre > m_pre)) (PreH3 : (0 < n_pre)) (PreH4 : (n_pre <= INT_MAX)) (PreH5 : (0 < m_pre)) (PreH6 : (m_pre <= INT_MAX)) (PreH7 : ((n_pre + m_pre ) <= INT_MAX)) (PreH8 : (problem_103_pre_z n_pre m_pre )) (PreH9 : (rounded_avg_safe_103 n_pre m_pre )) ,
+  (CharArray.undef_full retval 3 )
+  **  ((( &( "out" ) )) # Ptr  |-> retval)
+  **  ((( &( "num" ) )) # Int  |->_)
+  **  ((( &( "m" ) )) # Int  |-> m_pre)
+  **  ((( &( "n" ) )) # Int  |-> n_pre)
+|--
+  “ (45 <= INT_MAX) ” 
+  &&  “ ((INT_MIN) <= 45) ”
+.
+
+Definition rounded_avg_safety_wit_4 := 
+forall (m_pre: Z) (n_pre: Z) (retval: Z) (PreH1 : (retval <> 0)) (PreH2 : (n_pre > m_pre)) (PreH3 : (0 < n_pre)) (PreH4 : (n_pre <= INT_MAX)) (PreH5 : (0 < m_pre)) (PreH6 : (m_pre <= INT_MAX)) (PreH7 : ((n_pre + m_pre ) <= INT_MAX)) (PreH8 : (problem_103_pre_z n_pre m_pre )) (PreH9 : (rounded_avg_safe_103 n_pre m_pre )) ,
+  (CharArray.undef_seg retval (0 + 1 ) 3 )
+  **  (((retval + (0 * sizeof(CHAR) ) )) # Char  |-> 45)
+  **  ((( &( "out" ) )) # Ptr  |-> retval)
+  **  ((( &( "num" ) )) # Int  |->_)
+  **  ((( &( "m" ) )) # Int  |-> m_pre)
+  **  ((( &( "n" ) )) # Int  |-> n_pre)
+|--
+  “ (1 <= INT_MAX) ” 
+  &&  “ ((INT_MIN) <= 1) ”
+.
+
+Definition rounded_avg_safety_wit_5 := 
+forall (m_pre: Z) (n_pre: Z) (retval: Z) (PreH1 : (retval <> 0)) (PreH2 : (n_pre > m_pre)) (PreH3 : (0 < n_pre)) (PreH4 : (n_pre <= INT_MAX)) (PreH5 : (0 < m_pre)) (PreH6 : (m_pre <= INT_MAX)) (PreH7 : ((n_pre + m_pre ) <= INT_MAX)) (PreH8 : (problem_103_pre_z n_pre m_pre )) (PreH9 : (rounded_avg_safe_103 n_pre m_pre )) ,
+  (CharArray.undef_seg retval (0 + 1 ) 3 )
+  **  (((retval + (0 * sizeof(CHAR) ) )) # Char  |-> 45)
+  **  ((( &( "out" ) )) # Ptr  |-> retval)
+  **  ((( &( "num" ) )) # Int  |->_)
+  **  ((( &( "m" ) )) # Int  |-> m_pre)
+  **  ((( &( "n" ) )) # Int  |-> n_pre)
+|--
+  “ (49 <= INT_MAX) ” 
+  &&  “ ((INT_MIN) <= 49) ”
+.
+
+Definition rounded_avg_safety_wit_6 := 
+forall (m_pre: Z) (n_pre: Z) (retval: Z) (PreH1 : (retval <> 0)) (PreH2 : (n_pre > m_pre)) (PreH3 : (0 < n_pre)) (PreH4 : (n_pre <= INT_MAX)) (PreH5 : (0 < m_pre)) (PreH6 : (m_pre <= INT_MAX)) (PreH7 : ((n_pre + m_pre ) <= INT_MAX)) (PreH8 : (problem_103_pre_z n_pre m_pre )) (PreH9 : (rounded_avg_safe_103 n_pre m_pre )) ,
+  (CharArray.undef_seg retval (1 + 1 ) 3 )
+  **  (((retval + (1 * sizeof(CHAR) ) )) # Char  |-> 49)
+  **  (((retval + (0 * sizeof(CHAR) ) )) # Char  |-> 45)
+  **  ((( &( "out" ) )) # Ptr  |-> retval)
+  **  ((( &( "num" ) )) # Int  |->_)
+  **  ((( &( "m" ) )) # Int  |-> m_pre)
+  **  ((( &( "n" ) )) # Int  |-> n_pre)
+|--
+  “ (2 <= INT_MAX) ” 
+  &&  “ ((INT_MIN) <= 2) ”
+.
+
+Definition rounded_avg_safety_wit_7 := 
+forall (m_pre: Z) (n_pre: Z) (retval: Z) (PreH1 : (retval <> 0)) (PreH2 : (n_pre > m_pre)) (PreH3 : (0 < n_pre)) (PreH4 : (n_pre <= INT_MAX)) (PreH5 : (0 < m_pre)) (PreH6 : (m_pre <= INT_MAX)) (PreH7 : ((n_pre + m_pre ) <= INT_MAX)) (PreH8 : (problem_103_pre_z n_pre m_pre )) (PreH9 : (rounded_avg_safe_103 n_pre m_pre )) ,
+  (CharArray.undef_seg retval (1 + 1 ) 3 )
+  **  (((retval + (1 * sizeof(CHAR) ) )) # Char  |-> 49)
+  **  (((retval + (0 * sizeof(CHAR) ) )) # Char  |-> 45)
+  **  ((( &( "out" ) )) # Ptr  |-> retval)
+  **  ((( &( "num" ) )) # Int  |->_)
+  **  ((( &( "m" ) )) # Int  |-> m_pre)
+  **  ((( &( "n" ) )) # Int  |-> n_pre)
+|--
+  “ (0 <= INT_MAX) ” 
+  &&  “ ((INT_MIN) <= 0) ”
+.
+
+Definition rounded_avg_safety_wit_8 := 
+forall (m_pre: Z) (n_pre: Z) (PreH1 : (n_pre <= m_pre)) (PreH2 : (0 < n_pre)) (PreH3 : (n_pre <= INT_MAX)) (PreH4 : (0 < m_pre)) (PreH5 : (m_pre <= INT_MAX)) (PreH6 : ((n_pre + m_pre ) <= INT_MAX)) (PreH7 : (problem_103_pre_z n_pre m_pre )) (PreH8 : (rounded_avg_safe_103 n_pre m_pre )) ,
+  ((( &( "out" ) )) # Ptr  |->_)
+  **  ((( &( "num" ) )) # Int  |->_)
+  **  ((( &( "m" ) )) # Int  |-> m_pre)
+  **  ((( &( "n" ) )) # Int  |-> n_pre)
+|--
+  “ (((m_pre + n_pre ) <> (INT_MIN)) \/ (2 <> (-1))) ” 
+  &&  “ (2 <> 0) ”
+.
+
+Definition rounded_avg_safety_wit_9 := 
+forall (m_pre: Z) (n_pre: Z) (PreH1 : (n_pre <= m_pre)) (PreH2 : (0 < n_pre)) (PreH3 : (n_pre <= INT_MAX)) (PreH4 : (0 < m_pre)) (PreH5 : (m_pre <= INT_MAX)) (PreH6 : ((n_pre + m_pre ) <= INT_MAX)) (PreH7 : (problem_103_pre_z n_pre m_pre )) (PreH8 : (rounded_avg_safe_103 n_pre m_pre )) ,
+  ((( &( "out" ) )) # Ptr  |->_)
+  **  ((( &( "num" ) )) # Int  |->_)
+  **  ((( &( "m" ) )) # Int  |-> m_pre)
+  **  ((( &( "n" ) )) # Int  |-> n_pre)
+|--
+  “ ((m_pre + n_pre ) <= INT_MAX) ” 
+  &&  “ ((INT_MIN) <= (m_pre + n_pre )) ”
+.
+
+Definition rounded_avg_safety_wit_10 := 
+forall (m_pre: Z) (n_pre: Z) (PreH1 : (n_pre <= m_pre)) (PreH2 : (0 < n_pre)) (PreH3 : (n_pre <= INT_MAX)) (PreH4 : (0 < m_pre)) (PreH5 : (m_pre <= INT_MAX)) (PreH6 : ((n_pre + m_pre ) <= INT_MAX)) (PreH7 : (problem_103_pre_z n_pre m_pre )) (PreH8 : (rounded_avg_safe_103 n_pre m_pre )) ,
+  ((( &( "out" ) )) # Ptr  |->_)
+  **  ((( &( "num" ) )) # Int  |->_)
+  **  ((( &( "m" ) )) # Int  |-> m_pre)
+  **  ((( &( "n" ) )) # Int  |-> n_pre)
+|--
+  “ (2 <= INT_MAX) ” 
+  &&  “ ((INT_MIN) <= 2) ”
+.
+
+Definition rounded_avg_return_wit_1 := 
+(
+forall (m_pre: Z) (n_pre: Z) (out_l_2: (@list Z)) (len_2: Z) (retval: Z) (PreH1 : (len_2 = (Zlength (out_l_2)))) (PreH2 : (len_2 = (binary_length_z_103 (((m_pre + n_pre ) ÷ 2 ))))) (PreH3 : (out_l_2 = (binary_output_z_103 (((m_pre + n_pre ) ÷ 2 ))))) (PreH4 : (n_pre <= m_pre)) (PreH5 : (0 < n_pre)) (PreH6 : (n_pre <= INT_MAX)) (PreH7 : (0 < m_pre)) (PreH8 : (m_pre <= INT_MAX)) (PreH9 : ((n_pre + m_pre ) <= INT_MAX)) (PreH10 : (problem_103_pre_z n_pre m_pre )) (PreH11 : (rounded_avg_safe_103 n_pre m_pre )) ,
+  (CharArray.full retval (len_2 + 1 ) (app (out_l_2) ((cons (0) ((@nil Z))))) )
+|--
+  EX (out_l: (@list Z))  (len: Z) ,
+  “ (len = (Zlength (out_l))) ” 
+  &&  “ (problem_103_spec_z n_pre m_pre out_l ) ”
+  &&  (CharArray.full retval (len + 1 ) (app (out_l) ((cons (0) ((@nil Z))))) )
+) \/
+(
+forall (m_pre: Z) (n_pre: Z) (out_l_2: (@list Z)) (len_2: Z) (retval: Z) (PreH1 : (0 <= (len_2 + 1 ))) (PreH2 : (len_2 = (Zlength (out_l_2)))) (PreH3 : (len_2 = (binary_length_z_103 (((m_pre + n_pre ) ÷ 2 ))))) (PreH4 : (out_l_2 = (binary_output_z_103 (((m_pre + n_pre ) ÷ 2 ))))) (PreH5 : (n_pre <= m_pre)) (PreH6 : (0 < n_pre)) (PreH7 : (n_pre <= INT_MAX)) (PreH8 : (0 < m_pre)) (PreH9 : (m_pre <= INT_MAX)) (PreH10 : ((n_pre + m_pre ) <= INT_MAX)) (PreH11 : (problem_103_pre_z n_pre m_pre )) (PreH12 : (rounded_avg_safe_103 n_pre m_pre )) ,
+  (CharArray.full retval (len_2 + 1 ) (app (out_l_2) ((cons (0) ((@nil Z))))) )
+|--
+  EX (out_l: (@list Z)) ,
+  “ (problem_103_spec_z n_pre m_pre out_l ) ”
+  &&  (CharArray.full retval ((Zlength (out_l)) + 1 ) (app (out_l) ((cons (0) ((@nil Z))))) )
+).
+
+Definition rounded_avg_return_wit_2 := 
+(
+forall (m_pre: Z) (n_pre: Z) (retval: Z) (PreH1 : (retval <> 0)) (PreH2 : (n_pre > m_pre)) (PreH3 : (0 < n_pre)) (PreH4 : (n_pre <= INT_MAX)) (PreH5 : (0 < m_pre)) (PreH6 : (m_pre <= INT_MAX)) (PreH7 : ((n_pre + m_pre ) <= INT_MAX)) (PreH8 : (problem_103_pre_z n_pre m_pre )) (PreH9 : (rounded_avg_safe_103 n_pre m_pre )) ,
+  (CharArray.undef_seg retval (2 + 1 ) 3 )
+  **  (((retval + (2 * sizeof(CHAR) ) )) # Char  |-> 0)
+  **  (((retval + (1 * sizeof(CHAR) ) )) # Char  |-> 49)
+  **  (((retval + (0 * sizeof(CHAR) ) )) # Char  |-> 45)
+|--
+  EX (out_l: (@list Z))  (len: Z) ,
+  “ (len = (Zlength (out_l))) ” 
+  &&  “ (problem_103_spec_z n_pre m_pre out_l ) ”
+  &&  (CharArray.full retval (len + 1 ) (app (out_l) ((cons (0) ((@nil Z))))) )
+) \/
+(
+forall (m_pre: Z) (n_pre: Z) (retval: Z) (PreH1 : (retval <> 0)) (PreH2 : (n_pre > m_pre)) (PreH3 : (0 < n_pre)) (PreH4 : (n_pre <= INT_MAX)) (PreH5 : (0 < m_pre)) (PreH6 : (m_pre <= INT_MAX)) (PreH7 : ((n_pre + m_pre ) <= INT_MAX)) (PreH8 : (problem_103_pre_z n_pre m_pre )) (PreH9 : (rounded_avg_safe_103 n_pre m_pre )) ,
+  (((retval + (2 * sizeof(CHAR) ) )) # Char  |-> 0)
+  **  (((retval + (1 * sizeof(CHAR) ) )) # Char  |-> 49)
+  **  (((retval + (0 * sizeof(CHAR) ) )) # Char  |-> 45)
+|--
+  EX (out_l: (@list Z)) ,
+  “ (problem_103_spec_z n_pre m_pre out_l ) ”
+  &&  (CharArray.full retval ((Zlength (out_l)) + 1 ) (app (out_l) ((cons (0) ((@nil Z))))) )
+).
+
+Definition rounded_avg_partial_solve_wit_1_pure := 
+forall (m_pre: Z) (n_pre: Z) (PreH1 : (n_pre > m_pre)) (PreH2 : (0 < n_pre)) (PreH3 : (n_pre <= INT_MAX)) (PreH4 : (0 < m_pre)) (PreH5 : (m_pre <= INT_MAX)) (PreH6 : ((n_pre + m_pre ) <= INT_MAX)) (PreH7 : (problem_103_pre_z n_pre m_pre )) (PreH8 : (rounded_avg_safe_103 n_pre m_pre )) ,
+  ((( &( "out" ) )) # Ptr  |->_)
+  **  ((( &( "num" ) )) # Int  |->_)
+  **  ((( &( "m" ) )) # Int  |-> m_pre)
+  **  ((( &( "n" ) )) # Int  |-> n_pre)
+|--
+  “ (3 > 0) ” 
+  &&  “ (3 < INT_MAX) ”
+.
+
+Definition rounded_avg_partial_solve_wit_1_aux := 
+forall (m_pre: Z) (n_pre: Z) (PreH1 : (n_pre > m_pre)) (PreH2 : (0 < n_pre)) (PreH3 : (n_pre <= INT_MAX)) (PreH4 : (0 < m_pre)) (PreH5 : (m_pre <= INT_MAX)) (PreH6 : ((n_pre + m_pre ) <= INT_MAX)) (PreH7 : (problem_103_pre_z n_pre m_pre )) (PreH8 : (rounded_avg_safe_103 n_pre m_pre )) ,
+  TT && emp 
+|--
+  “ (3 > 0) ” 
+  &&  “ (3 < INT_MAX) ” 
+  &&  “ (n_pre > m_pre) ” 
+  &&  “ (0 < n_pre) ” 
+  &&  “ (n_pre <= INT_MAX) ” 
+  &&  “ (0 < m_pre) ” 
+  &&  “ (m_pre <= INT_MAX) ” 
+  &&  “ ((n_pre + m_pre ) <= INT_MAX) ” 
+  &&  “ (problem_103_pre_z n_pre m_pre ) ” 
+  &&  “ (rounded_avg_safe_103 n_pre m_pre ) ”
+  &&  emp
+.
+
+Definition rounded_avg_partial_solve_wit_1 := rounded_avg_partial_solve_wit_1_pure -> rounded_avg_partial_solve_wit_1_aux.
+
+Definition rounded_avg_partial_solve_wit_2 := 
+forall (m_pre: Z) (n_pre: Z) (retval: Z) (PreH1 : (retval <> 0)) (PreH2 : (n_pre > m_pre)) (PreH3 : (0 < n_pre)) (PreH4 : (n_pre <= INT_MAX)) (PreH5 : (0 < m_pre)) (PreH6 : (m_pre <= INT_MAX)) (PreH7 : ((n_pre + m_pre ) <= INT_MAX)) (PreH8 : (problem_103_pre_z n_pre m_pre )) (PreH9 : (rounded_avg_safe_103 n_pre m_pre )) ,
+  (CharArray.undef_full retval 3 )
+|--
+  “ (retval <> 0) ” 
+  &&  “ (n_pre > m_pre) ” 
+  &&  “ (0 < n_pre) ” 
+  &&  “ (n_pre <= INT_MAX) ” 
+  &&  “ (0 < m_pre) ” 
+  &&  “ (m_pre <= INT_MAX) ” 
+  &&  “ ((n_pre + m_pre ) <= INT_MAX) ” 
+  &&  “ (problem_103_pre_z n_pre m_pre ) ” 
+  &&  “ (rounded_avg_safe_103 n_pre m_pre ) ”
+  &&  (((retval + (0 * sizeof(CHAR) ) )) # Char  |->_)
+  **  (CharArray.undef_missing_i retval 0 0 3 )
+.
+
+Definition rounded_avg_partial_solve_wit_3 := 
+forall (m_pre: Z) (n_pre: Z) (retval: Z) (PreH1 : (retval <> 0)) (PreH2 : (n_pre > m_pre)) (PreH3 : (0 < n_pre)) (PreH4 : (n_pre <= INT_MAX)) (PreH5 : (0 < m_pre)) (PreH6 : (m_pre <= INT_MAX)) (PreH7 : ((n_pre + m_pre ) <= INT_MAX)) (PreH8 : (problem_103_pre_z n_pre m_pre )) (PreH9 : (rounded_avg_safe_103 n_pre m_pre )) ,
+  (CharArray.undef_seg retval (0 + 1 ) 3 )
+  **  (((retval + (0 * sizeof(CHAR) ) )) # Char  |-> 45)
+|--
+  “ (retval <> 0) ” 
+  &&  “ (n_pre > m_pre) ” 
+  &&  “ (0 < n_pre) ” 
+  &&  “ (n_pre <= INT_MAX) ” 
+  &&  “ (0 < m_pre) ” 
+  &&  “ (m_pre <= INT_MAX) ” 
+  &&  “ ((n_pre + m_pre ) <= INT_MAX) ” 
+  &&  “ (problem_103_pre_z n_pre m_pre ) ” 
+  &&  “ (rounded_avg_safe_103 n_pre m_pre ) ”
+  &&  (((retval + (1 * sizeof(CHAR) ) )) # Char  |->_)
+  **  (CharArray.undef_missing_i retval 1 (0 + 1 ) 3 )
+  **  (((retval + (0 * sizeof(CHAR) ) )) # Char  |-> 45)
+.
+
+Definition rounded_avg_partial_solve_wit_4 := 
+forall (m_pre: Z) (n_pre: Z) (retval: Z) (PreH1 : (retval <> 0)) (PreH2 : (n_pre > m_pre)) (PreH3 : (0 < n_pre)) (PreH4 : (n_pre <= INT_MAX)) (PreH5 : (0 < m_pre)) (PreH6 : (m_pre <= INT_MAX)) (PreH7 : ((n_pre + m_pre ) <= INT_MAX)) (PreH8 : (problem_103_pre_z n_pre m_pre )) (PreH9 : (rounded_avg_safe_103 n_pre m_pre )) ,
+  (CharArray.undef_seg retval (1 + 1 ) 3 )
+  **  (((retval + (1 * sizeof(CHAR) ) )) # Char  |-> 49)
+  **  (((retval + (0 * sizeof(CHAR) ) )) # Char  |-> 45)
+|--
+  “ (retval <> 0) ” 
+  &&  “ (n_pre > m_pre) ” 
+  &&  “ (0 < n_pre) ” 
+  &&  “ (n_pre <= INT_MAX) ” 
+  &&  “ (0 < m_pre) ” 
+  &&  “ (m_pre <= INT_MAX) ” 
+  &&  “ ((n_pre + m_pre ) <= INT_MAX) ” 
+  &&  “ (problem_103_pre_z n_pre m_pre ) ” 
+  &&  “ (rounded_avg_safe_103 n_pre m_pre ) ”
+  &&  (((retval + (2 * sizeof(CHAR) ) )) # Char  |->_)
+  **  (CharArray.undef_missing_i retval 2 (1 + 1 ) 3 )
+  **  (((retval + (1 * sizeof(CHAR) ) )) # Char  |-> 49)
+  **  (((retval + (0 * sizeof(CHAR) ) )) # Char  |-> 45)
+.
+
+Definition rounded_avg_partial_solve_wit_5_pure := 
+(
+forall (m_pre: Z) (n_pre: Z) (PreH1 : (n_pre <= m_pre)) (PreH2 : (0 < n_pre)) (PreH3 : (n_pre <= INT_MAX)) (PreH4 : (0 < m_pre)) (PreH5 : (m_pre <= INT_MAX)) (PreH6 : ((n_pre + m_pre ) <= INT_MAX)) (PreH7 : (problem_103_pre_z n_pre m_pre )) (PreH8 : (rounded_avg_safe_103 n_pre m_pre )) ,
+  ((( &( "out" ) )) # Ptr  |->_)
+  **  ((( &( "num" ) )) # Int  |-> ((m_pre + n_pre ) ÷ 2 ))
+  **  ((( &( "m" ) )) # Int  |-> m_pre)
+  **  ((( &( "n" ) )) # Int  |-> n_pre)
+|--
+  “ (binary_safe_103 ((m_pre + n_pre ) ÷ 2 ) ) ” 
+  &&  “ (((m_pre + n_pre ) ÷ 2 ) <= INT_MAX) ” 
+  &&  “ (0 <= ((m_pre + n_pre ) ÷ 2 )) ”
+) \/
+(
+forall (m_pre: Z) (n_pre: Z) (PreH1 : (((m_pre + n_pre ) ÷ 2 ) <= INT_MAX)) (PreH2 : (n_pre >= INT_MIN)) (PreH3 : (m_pre >= INT_MIN)) (PreH4 : (((m_pre + n_pre ) ÷ 2 ) >= INT_MIN)) (PreH5 : (n_pre <= m_pre)) (PreH6 : (0 < n_pre)) (PreH7 : (n_pre <= INT_MAX)) (PreH8 : (0 < m_pre)) (PreH9 : (m_pre <= INT_MAX)) (PreH10 : ((n_pre + m_pre ) <= INT_MAX)) (PreH11 : (problem_103_pre_z n_pre m_pre )) (PreH12 : (rounded_avg_safe_103 n_pre m_pre )) ,
+  ((( &( "out" ) )) # Ptr  |->_)
+  **  ((( &( "num" ) )) # Int  |-> ((m_pre + n_pre ) ÷ 2 ))
+  **  ((( &( "m" ) )) # Int  |-> m_pre)
+  **  ((( &( "n" ) )) # Int  |-> n_pre)
+|--
+  “ (0 <= ((m_pre + n_pre ) ÷ 2 )) ” 
+  &&  “ (binary_safe_103 ((m_pre + n_pre ) ÷ 2 ) ) ”
+).
+
+Definition rounded_avg_partial_solve_wit_5_pure_split_goal_1 := 
+forall (m_pre: Z) (n_pre: Z) (PreH1 : (((m_pre + n_pre ) ÷ 2 ) <= INT_MAX)) (PreH2 : (n_pre >= INT_MIN)) (PreH3 : (m_pre >= INT_MIN)) (PreH4 : (((m_pre + n_pre ) ÷ 2 ) >= INT_MIN)) (PreH5 : (n_pre <= m_pre)) (PreH6 : (0 < n_pre)) (PreH7 : (n_pre <= INT_MAX)) (PreH8 : (0 < m_pre)) (PreH9 : (m_pre <= INT_MAX)) (PreH10 : ((n_pre + m_pre ) <= INT_MAX)) (PreH11 : (problem_103_pre_z n_pre m_pre )) (PreH12 : (rounded_avg_safe_103 n_pre m_pre )) ,
+  ((( &( "out" ) )) # Ptr  |->_)
+  **  ((( &( "num" ) )) # Int  |-> ((m_pre + n_pre ) ÷ 2 ))
+  **  ((( &( "m" ) )) # Int  |-> m_pre)
+  **  ((( &( "n" ) )) # Int  |-> n_pre)
+|--
+  “ (0 <= ((m_pre + n_pre ) ÷ 2 )) ”
+.
+
+Definition rounded_avg_partial_solve_wit_5_pure_split_goal_2 := 
+forall (m_pre: Z) (n_pre: Z) (PreH1 : (((m_pre + n_pre ) ÷ 2 ) <= INT_MAX)) (PreH2 : (n_pre >= INT_MIN)) (PreH3 : (m_pre >= INT_MIN)) (PreH4 : (((m_pre + n_pre ) ÷ 2 ) >= INT_MIN)) (PreH5 : (n_pre <= m_pre)) (PreH6 : (0 < n_pre)) (PreH7 : (n_pre <= INT_MAX)) (PreH8 : (0 < m_pre)) (PreH9 : (m_pre <= INT_MAX)) (PreH10 : ((n_pre + m_pre ) <= INT_MAX)) (PreH11 : (problem_103_pre_z n_pre m_pre )) (PreH12 : (rounded_avg_safe_103 n_pre m_pre )) ,
+  ((( &( "out" ) )) # Ptr  |->_)
+  **  ((( &( "num" ) )) # Int  |-> ((m_pre + n_pre ) ÷ 2 ))
+  **  ((( &( "m" ) )) # Int  |-> m_pre)
+  **  ((( &( "n" ) )) # Int  |-> n_pre)
+|--
+  “ (binary_safe_103 ((m_pre + n_pre ) ÷ 2 ) ) ”
+.
+
+Definition rounded_avg_partial_solve_wit_5_aux := 
+forall (m_pre: Z) (n_pre: Z) (PreH1 : (n_pre <= m_pre)) (PreH2 : (0 < n_pre)) (PreH3 : (n_pre <= INT_MAX)) (PreH4 : (0 < m_pre)) (PreH5 : (m_pre <= INT_MAX)) (PreH6 : ((n_pre + m_pre ) <= INT_MAX)) (PreH7 : (problem_103_pre_z n_pre m_pre )) (PreH8 : (rounded_avg_safe_103 n_pre m_pre )) ,
+  TT && emp 
+|--
+  “ (binary_safe_103 ((m_pre + n_pre ) ÷ 2 ) ) ” 
+  &&  “ (((m_pre + n_pre ) ÷ 2 ) <= INT_MAX) ” 
+  &&  “ (0 <= ((m_pre + n_pre ) ÷ 2 )) ” 
+  &&  “ (n_pre <= m_pre) ” 
+  &&  “ (0 < n_pre) ” 
+  &&  “ (n_pre <= INT_MAX) ” 
+  &&  “ (0 < m_pre) ” 
+  &&  “ (m_pre <= INT_MAX) ” 
+  &&  “ ((n_pre + m_pre ) <= INT_MAX) ” 
+  &&  “ (problem_103_pre_z n_pre m_pre ) ” 
+  &&  “ (rounded_avg_safe_103 n_pre m_pre ) ”
+  &&  emp
+.
+
+Definition rounded_avg_partial_solve_wit_5 := rounded_avg_partial_solve_wit_5_pure -> rounded_avg_partial_solve_wit_5_aux.
+
+Module Type VC_Correct.
+
+Include char_array_Strategy_Correct.
+Include string_Strategy_Correct.
+
+Axiom proof_of_to_binary_string_safety_wit_1 : to_binary_string_safety_wit_1.
+Axiom proof_of_to_binary_string_safety_wit_2 : to_binary_string_safety_wit_2.
+Axiom proof_of_to_binary_string_safety_wit_3 : to_binary_string_safety_wit_3.
+Axiom proof_of_to_binary_string_safety_wit_4 : to_binary_string_safety_wit_4.
+Axiom proof_of_to_binary_string_safety_wit_5 : to_binary_string_safety_wit_5.
+Axiom proof_of_to_binary_string_safety_wit_6 : to_binary_string_safety_wit_6.
+Axiom proof_of_to_binary_string_safety_wit_7 : to_binary_string_safety_wit_7.
+Axiom proof_of_to_binary_string_safety_wit_8 : to_binary_string_safety_wit_8.
+Axiom proof_of_to_binary_string_safety_wit_9 : to_binary_string_safety_wit_9.
+Axiom proof_of_to_binary_string_safety_wit_10 : to_binary_string_safety_wit_10.
+Axiom proof_of_to_binary_string_safety_wit_11 : to_binary_string_safety_wit_11.
+Axiom proof_of_to_binary_string_safety_wit_12 : to_binary_string_safety_wit_12.
+Axiom proof_of_to_binary_string_safety_wit_13 : to_binary_string_safety_wit_13.
+Axiom proof_of_to_binary_string_safety_wit_14 : to_binary_string_safety_wit_14.
+Axiom proof_of_to_binary_string_safety_wit_15 : to_binary_string_safety_wit_15.
+Axiom proof_of_to_binary_string_safety_wit_16 : to_binary_string_safety_wit_16.
+Axiom proof_of_to_binary_string_safety_wit_17 : to_binary_string_safety_wit_17.
+Axiom proof_of_to_binary_string_safety_wit_18 : to_binary_string_safety_wit_18.
+Axiom proof_of_to_binary_string_safety_wit_19 : to_binary_string_safety_wit_19.
+Axiom proof_of_to_binary_string_safety_wit_20 : to_binary_string_safety_wit_20.
+Axiom proof_of_to_binary_string_safety_wit_21 : to_binary_string_safety_wit_21.
+Axiom proof_of_to_binary_string_safety_wit_22 : to_binary_string_safety_wit_22.
+Axiom proof_of_to_binary_string_safety_wit_23 : to_binary_string_safety_wit_23.
+Axiom proof_of_to_binary_string_safety_wit_24 : to_binary_string_safety_wit_24.
+Axiom proof_of_to_binary_string_safety_wit_25 : to_binary_string_safety_wit_25.
+Axiom proof_of_to_binary_string_safety_wit_26 : to_binary_string_safety_wit_26.
+Axiom proof_of_to_binary_string_safety_wit_27 : to_binary_string_safety_wit_27.
+Axiom proof_of_to_binary_string_entail_wit_1 : to_binary_string_entail_wit_1.
+Axiom proof_of_to_binary_string_entail_wit_2 : to_binary_string_entail_wit_2.
+Axiom proof_of_to_binary_string_entail_wit_3 : to_binary_string_entail_wit_3.
+Axiom proof_of_to_binary_string_entail_wit_4 : to_binary_string_entail_wit_4.
+Axiom proof_of_to_binary_string_entail_wit_5 : to_binary_string_entail_wit_5.
+Axiom proof_of_to_binary_string_entail_wit_6 : to_binary_string_entail_wit_6.
+Axiom proof_of_to_binary_string_entail_wit_7 : to_binary_string_entail_wit_7.
+Axiom proof_of_to_binary_string_entail_wit_8 : to_binary_string_entail_wit_8.
+Axiom proof_of_to_binary_string_entail_wit_9 : to_binary_string_entail_wit_9.
+Axiom proof_of_to_binary_string_return_wit_1 : to_binary_string_return_wit_1.
+Axiom proof_of_to_binary_string_return_wit_2 : to_binary_string_return_wit_2.
+Axiom proof_of_to_binary_string_partial_solve_wit_1_pure : to_binary_string_partial_solve_wit_1_pure.
+Axiom proof_of_to_binary_string_partial_solve_wit_1 : to_binary_string_partial_solve_wit_1.
+Axiom proof_of_to_binary_string_partial_solve_wit_2 : to_binary_string_partial_solve_wit_2.
+Axiom proof_of_to_binary_string_partial_solve_wit_3 : to_binary_string_partial_solve_wit_3.
+Axiom proof_of_to_binary_string_partial_solve_wit_4_pure : to_binary_string_partial_solve_wit_4_pure.
+Axiom proof_of_to_binary_string_partial_solve_wit_4 : to_binary_string_partial_solve_wit_4.
+Axiom proof_of_to_binary_string_partial_solve_wit_5 : to_binary_string_partial_solve_wit_5.
+Axiom proof_of_to_binary_string_partial_solve_wit_6 : to_binary_string_partial_solve_wit_6.
+Axiom proof_of_rounded_avg_safety_wit_1 : rounded_avg_safety_wit_1.
+Axiom proof_of_rounded_avg_safety_wit_2 : rounded_avg_safety_wit_2.
+Axiom proof_of_rounded_avg_safety_wit_3 : rounded_avg_safety_wit_3.
+Axiom proof_of_rounded_avg_safety_wit_4 : rounded_avg_safety_wit_4.
+Axiom proof_of_rounded_avg_safety_wit_5 : rounded_avg_safety_wit_5.
+Axiom proof_of_rounded_avg_safety_wit_6 : rounded_avg_safety_wit_6.
+Axiom proof_of_rounded_avg_safety_wit_7 : rounded_avg_safety_wit_7.
+Axiom proof_of_rounded_avg_safety_wit_8 : rounded_avg_safety_wit_8.
+Axiom proof_of_rounded_avg_safety_wit_9 : rounded_avg_safety_wit_9.
+Axiom proof_of_rounded_avg_safety_wit_10 : rounded_avg_safety_wit_10.
+Axiom proof_of_rounded_avg_return_wit_1 : rounded_avg_return_wit_1.
+Axiom proof_of_rounded_avg_return_wit_2 : rounded_avg_return_wit_2.
+Axiom proof_of_rounded_avg_partial_solve_wit_1_pure : rounded_avg_partial_solve_wit_1_pure.
+Axiom proof_of_rounded_avg_partial_solve_wit_1 : rounded_avg_partial_solve_wit_1.
+Axiom proof_of_rounded_avg_partial_solve_wit_2 : rounded_avg_partial_solve_wit_2.
+Axiom proof_of_rounded_avg_partial_solve_wit_3 : rounded_avg_partial_solve_wit_3.
+Axiom proof_of_rounded_avg_partial_solve_wit_4 : rounded_avg_partial_solve_wit_4.
+Axiom proof_of_rounded_avg_partial_solve_wit_5_pure : rounded_avg_partial_solve_wit_5_pure.
+Axiom proof_of_rounded_avg_partial_solve_wit_5 : rounded_avg_partial_solve_wit_5.
+
+End VC_Correct.
