QCP_examples/humaneval/spec_logic_rewrite_c_files/C_103_goal_check.v
@@ -1,0 +1,8 @@
+From SimpleC.EE Require Import C_103_goal C_103_proof_auto C_103_proof_manual.
+
+Module VC_Correctness : VC_Correct.
+  Include char_array_strategy_proof.
+  Include string_strategy_proof.
+  Include C_103_proof_auto.
+  Include C_103_proof_manual.
+End VC_Correctness.
