QCP_examples/humaneval/spec_logic_rewrite_c_files/C_103_proof_manual.v
@@ -18,5 +18,244 @@ Local Open Scope sets.
 Local Open Scope string_scope.
 Local Open Scope list.
 Import naive_C_Rules.
+Require Import SimpleC.StdLib.string_lib.
+Require Import coins_103.
 Local Open Scope sac.
 
+Lemma proof_of_to_binary_string_safety_wit_10 : to_binary_string_safety_wit_10.
+Proof.
+  left; pre_process; entailer!.
+  pose proof (binary_safe_length_bound_103 num_pre PreH7) as Hlen.
+  unfold binary_count_state_z_103 in PreH8.
+  destruct PreH8 as (_ & _ & Hcount).
+  pose proof (Zlength_nonneg (binary_bits_pos_z_103 x)).
+  assert (Hlen_eq : binary_length_z_103 num_pre =
+                    Zlength (binary_bits_pos_z_103 num_pre)).
+  {
+    unfold binary_length_z_103, binary_output_z_103,
+      binary_bits_z_103, binary_bits_pos_z_103.
+    destruct num_pre; try lia; simpl.
+    rewrite !Zlength_correct, length_map, length_rev.
+    reflexivity.
+  }
+  entailer!.
+Qed.
+
+Lemma proof_of_to_binary_string_safety_wit_14 : to_binary_string_safety_wit_14.
+Proof.
+  left; pre_process; entailer!.
+  pose proof (binary_safe_length_bound_103 num_pre PreH7).
+  entailer!.
+Qed.
+
+Lemma proof_of_to_binary_string_safety_wit_20 : to_binary_string_safety_wit_20.
+Proof.
+  left; intros.
+  pose proof (Z.rem_bound_pos num 2 ltac:(lia) ltac:(lia)).
+  entailer!.
+Qed.
+
+Lemma proof_of_to_binary_string_entail_wit_1 : to_binary_string_entail_wit_1.
+Proof.
+  left; intros.
+  pose proof (binary_safe_count_initial_103 num_pre PreH4).
+  entailer!.
+Qed.
+
+Lemma proof_of_to_binary_string_entail_wit_2 : to_binary_string_entail_wit_2.
+Proof.
+  left; intros.
+  pose proof (binary_safe_count_step_103
+    num_pre x bits PreH7 PreH8 ltac:(lia)) as Hstep.
+  assert (0 <= x ÷ 2) by (apply Z.quot_pos; lia).
+  entailer!.
+Qed.
+
+Lemma proof_of_to_binary_string_entail_wit_3 : to_binary_string_entail_wit_3.
+Proof.
+  left; intros.
+  assert (x = 0) by lia; subst x.
+  pose proof (binary_safe_count_final_103
+    num_pre bits PreH7 PreH2 PreH8) as Hbits.
+  pose proof (binary_safe_length_pos_103
+    num_pre bits PreH7 PreH2 Hbits) as Hpos.
+  entailer!.
+Qed.
+
+Lemma proof_of_to_binary_string_entail_wit_4 : to_binary_string_entail_wit_4.
+Proof.
+  left; intros.
+  pose proof (binary_safe_backfill_initial_103
+    num_pre bits PreH8 PreH2 PreH5) as Hstate.
+  entailer!.
+  rewrite derivable1_sepcon_comm.
+  apply derivable1_sepcon_mono.
+  - change (CharArray.undef_missing_i retval bits 0 (bits + 1) |--
+            CharArray.undef_seg retval 0 bits).
+    pose proof (CharArray.undef_missing_i_to_undef_seg_tail
+      retval 0 (bits + 1)) as Htail.
+    replace (bits + 1 - 1) with bits in Htail by lia.
+    apply Htail; lia.
+  - apply CharArray.seg_single.
+Qed.
+
+Lemma proof_of_to_binary_string_entail_wit_5 : to_binary_string_entail_wit_5.
+Proof.
+  left; intros.
+  subst x bits.
+  Exists (cons 0 nil).
+  entailer!.
+  change (1 = binary_length_z_103 num_pre + 1 -
+              binary_length_z_103 num_pre).
+  ring.
+Qed.
+
+Lemma proof_of_to_binary_string_entail_wit_6 : to_binary_string_entail_wit_6.
+Proof.
+  left; intros.
+  pose proof (binary_safe_backfill_step_103
+    num_pre num bits suffix_2 PreH10 PreH11 ltac:(lia)) as (Hbits & _).
+  Exists suffix_2.
+  entailer!.
+Qed.
+
+Lemma proof_of_to_binary_string_entail_wit_7 : to_binary_string_entail_wit_7.
+Proof.
+  left; intros.
+  pose proof (binary_safe_backfill_step_103
+    num_pre num bits suffix_2 PreH9 PreH10 PreH1)
+    as (_ & Hchar & Hnext).
+  Exists suffix_2.
+  entailer!.
+  - rewrite (signed_last_nbits_eq (48 + num % 2) 8) by lia.
+    sep_apply_l_atomic (CharArray.seg_single out (bits - 1)
+      (48 + num % 2)).
+    replace (bits - 1 + 1) with bits by lia.
+    sep_apply_l_atomic
+      (CharArray.undef_missing_i_to_undef_seg_tail out 0 bits).
+    + entailer!.
+    + replace (bits + 0 - 1) with (bits - 1) by lia.
+      cancel (CharArray.undef_seg out 0 (bits - 1)).
+      sep_apply_l_atomic (CharArray.seg_merge_to_seg
+        out (bits - 1) bits (binary_length_z_103 num_pre + 1)
+        (48 + num % 2 :: nil) suffix_2).
+      * entailer!.
+      * simpl; entailer!.
+  - rewrite Zlength_cons; lia.
+Qed.
+
+Lemma proof_of_to_binary_string_entail_wit_8 : to_binary_string_entail_wit_8.
+Proof.
+  left; intros.
+  Exists (cons (48 + num % 2) suffix_2).
+  assert (Hquot_nonneg : 0 <= num ÷ 2) by (apply Z.quot_pos; lia).
+  assert (Hquot_le : num ÷ 2 <= num_pre).
+  { eapply Z.quot_le_upper_bound; lia. }
+  entailer!.
+Qed.
+
+Lemma proof_of_to_binary_string_entail_wit_9 : to_binary_string_entail_wit_9.
+Proof.
+  left; intros.
+  assert (Hnum0 : num = 0) by lia; subst num.
+  pose proof (binary_backfill_zero_pos_103
+    num_pre bits suffix_2 PreH11) as Hbits; subst bits.
+  pose proof (binary_safe_backfill_final_103
+    num_pre suffix_2 PreH10 PreH11) as Hsuffix; subst suffix_2.
+  Exists (app (binary_output_z_103 num_pre) (0 :: nil)).
+  entailer!.
+  rewrite (CharArray.undef_seg_empty out 0).
+  entailer!.
+Qed.
+
+Lemma proof_of_to_binary_string_return_wit_1 : to_binary_string_return_wit_1.
+Proof.
+  left; intros.
+  subst suffix.
+  Exists (binary_output_z_103 num_pre) (binary_length_z_103 num_pre).
+  unfold binary_length_z_103.
+  entailer!.
+Qed.
+
+Lemma proof_of_to_binary_string_return_wit_2 : to_binary_string_return_wit_2.
+Proof.
+  left; intros.
+  subst num_pre.
+  pose proof (binary_safe_zero_output_103 0 PreH5 eq_refl) as Hzero.
+  Exists (binary_output_z_103 0) (binary_length_z_103 0).
+  rewrite Hzero in *.
+  entailer!.
+  rewrite (CharArray.undef_seg_empty retval 2).
+  sep_apply_l_atomic (CharArray.seg_single retval 1 0).
+  sep_apply_l_atomic (CharArray.seg_single retval 0 48).
+  sep_apply_l_atomic (CharArray.seg_merge_to_seg
+    retval 0 1 2 (48 :: nil) (0 :: nil)).
+  - entailer!.
+  - simpl.
+    sep_apply_l_atomic
+      (CharArray.seg_to_full retval 0 2 (48 :: 0 :: nil)).
+    replace (retval + 0 * sizeof(CHAR)) with retval by lia.
+    replace (2 - 0) with 2 by lia.
+    entailer!.
+Qed.
+
+Lemma proof_of_to_binary_string_partial_solve_wit_4_pure :
+  to_binary_string_partial_solve_wit_4_pure.
+Proof.
+  left; intros.
+  pose proof (binary_safe_length_bound_103 num_pre PreH7).
+  entailer!.
+Qed.
+
+Lemma proof_of_rounded_avg_return_wit_1 : rounded_avg_return_wit_1.
+Proof.
+  left; intros.
+  replace (m_pre + n_pre) with (n_pre + m_pre) in * by lia.
+  pose proof (rounded_avg_safe_use_103
+    n_pre m_pre PreH11 PreH4) as Hsafe.
+  cbn in Hsafe.
+  destruct Hsafe as (Havg & Hdiv & Hbinary).
+  subst out_l_2.
+  pose proof (problem_103_spec_z_binary
+    n_pre m_pre ((n_pre + m_pre) ÷ 2)
+    PreH4 ltac:(lia) Hdiv) as Hspec.
+  Exists (binary_output_z_103 ((n_pre + m_pre) ÷ 2)) len_2.
+  entailer!.
+Qed.
+
+Lemma proof_of_rounded_avg_return_wit_2 : rounded_avg_return_wit_2.
+Proof.
+  left; intros.
+  pose proof (problem_103_spec_z_neg n_pre m_pre PreH2) as Hspec.
+  Exists (45 :: 49 :: nil) 2.
+  entailer!.
+  rewrite (CharArray.undef_seg_empty retval 3).
+  sep_apply_l_atomic (CharArray.seg_single retval 2 0).
+  sep_apply_l_atomic (CharArray.seg_single retval 1 49).
+  sep_apply_l_atomic (CharArray.seg_single retval 0 45).
+  sep_apply_l_atomic (CharArray.seg_merge_to_seg
+    retval 0 1 2 (45 :: nil) (49 :: nil)).
+  - entailer!.
+  - simpl.
+    sep_apply_l_atomic (CharArray.seg_merge_to_seg
+      retval 0 2 3 (45 :: 49 :: nil) (0 :: nil)).
+    + entailer!.
+    + simpl.
+      sep_apply_l_atomic
+        (CharArray.seg_to_full retval 0 3 (45 :: 49 :: 0 :: nil)).
+      replace (retval + 0 * sizeof(CHAR)) with retval by lia.
+      replace (3 - 0) with 3 by lia.
+      entailer!.
+Qed.
+
+Lemma proof_of_rounded_avg_partial_solve_wit_5_pure :
+  rounded_avg_partial_solve_wit_5_pure.
+Proof.
+  left; intros.
+  replace (m_pre + n_pre) with (n_pre + m_pre) in * by lia.
+  pose proof (rounded_avg_safe_use_103
+    n_pre m_pre PreH8 PreH1) as Hsafe.
+  cbn in Hsafe.
+  destruct Hsafe as (Havg & Hdiv & Hbinary).
+  entailer!.
+Qed.
