QCP_examples/humaneval/spec_logic_rewrite_c_files/coins_103.v
@@ -1,0 +1,349 @@
+Load "../spec/103".
+
+Require Import Coq.ZArith.ZArith.
+Require Import Coq.Lists.List.
+Require Import Coq.Strings.String.
+Require Import Coq.Strings.Ascii.
+Require Import Coq.micromega.Lia.
+From AUXLib Require Import ListLib.
+From SimpleC.SL Require Import IntLib.
+
+Import ListNotations.
+
+Local Open Scope Z_scope.
+Local Open Scope string_scope.
+Local Open Scope list_scope.
+
+Definition ascii_of_z_103 (z : Z) : ascii :=
+  ascii_of_nat (Z.to_nat z).
+
+Fixpoint string_of_list_z_103 (l : list Z) : string :=
+  match l with
+  | [] => EmptyString
+  | c :: rest => String (ascii_of_z_103 c) (string_of_list_z_103 rest)
+  end.
+
+Definition problem_103_pre_z (n m : Z) : Prop :=
+  problem_103_pre n m.
+
+Definition problem_103_spec_z (n m : Z) (output : list Z) : Prop :=
+  problem_103_spec n m (string_of_list_z_103 output).
+
+Fixpoint positive_bits_103 (p : positive) : list Z :=
+  match p with
+  | xH => [1]
+  | xO q => 0 :: positive_bits_103 q
+  | xI q => 1 :: positive_bits_103 q
+  end.
+
+Definition binary_bits_pos_z_103 (n : Z) : list Z :=
+  match n with
+  | Zpos p => positive_bits_103 p
+  | _ => []
+  end.
+
+Definition binary_bits_z_103 (n : Z) : list Z :=
+  match n with
+  | Z0 => [0]
+  | Zpos p => positive_bits_103 p
+  | Zneg _ => []
+  end.
+
+Definition bit_code_z_103 (b : Z) : Z := 48 + b.
+
+Definition binary_output_z_103 (n : Z) : list Z :=
+  map bit_code_z_103 (rev (binary_bits_z_103 n)).
+
+Definition binary_length_z_103 (n : Z) : Z :=
+  Zlength (binary_output_z_103 n).
+
+Definition binary_count_state_z_103 (orig x bits : Z) : Prop :=
+  0 <= x /\
+  0 <= bits /\
+  bits + Zlength (binary_bits_pos_z_103 x) =
+    Zlength (binary_bits_pos_z_103 orig).
+
+Definition binary_backfill_state_z_103
+    (orig rem pos : Z) (suffix : list Z) : Prop :=
+  exists done,
+    0 < orig /\
+    0 <= rem <= orig /\
+    0 <= pos <= binary_length_z_103 orig /\
+    binary_bits_pos_z_103 orig = done ++ binary_bits_pos_z_103 rem /\
+    pos = binary_length_z_103 orig - Zlength done /\
+    suffix = map bit_code_z_103 (rev done) ++ [0].
+
+(* This predicate contains only arithmetic, loop-transition, and allocation
+   safety facts for the existing C helper.  The original problem spec is
+   connected separately by proved lemmas below. *)
+Definition binary_safe_103 (num : Z) : Prop :=
+  0 <= num <= INT_MAX /\
+  0 < binary_length_z_103 num + 1 < INT_MAX /\
+  binary_output_z_103 0 = [48] /\
+  binary_count_state_z_103 num num 0 /\
+  (forall x bits,
+      binary_count_state_z_103 num x bits ->
+      0 < x ->
+      binary_count_state_z_103 num (Z.quot x 2) (bits + 1)) /\
+  (forall bits,
+      0 < num ->
+      binary_count_state_z_103 num 0 bits ->
+      bits = binary_length_z_103 num) /\
+  (forall bits,
+      0 < num ->
+      bits = binary_length_z_103 num ->
+      1 <= bits) /\
+  (forall bits,
+      0 < num ->
+      bits = binary_length_z_103 num ->
+      binary_backfill_state_z_103 num num bits [0]) /\
+  (forall rem pos suffix,
+      binary_backfill_state_z_103 num rem pos suffix ->
+      0 < rem ->
+      0 < pos /\
+      0 <= 48 + Z.rem rem 2 <= 127 /\
+      binary_backfill_state_z_103
+        num (Z.quot rem 2) (pos - 1)
+        ((48 + Z.rem rem 2) :: suffix)) /\
+  (forall suffix,
+      binary_backfill_state_z_103 num 0 0 suffix ->
+      suffix = binary_output_z_103 num ++ [0]).
+
+Definition rounded_avg_safe_103 (n m : Z) : Prop :=
+  n <= m ->
+  let avg := Z.quot (n + m) 2 in
+  0 < avg <= INT_MAX /\
+  Z.quot (n + m) 2 = (n + m) / 2 /\
+  binary_safe_103 avg.
+
+Lemma binary_safe_length_bound_103 : forall n,
+  binary_safe_103 n ->
+  0 < binary_length_z_103 n + 1 < INT_MAX.
+Proof. intros n H; unfold binary_safe_103 in H; tauto. Qed.
+
+Lemma binary_safe_count_initial_103 : forall n,
+  binary_safe_103 n ->
+  binary_count_state_z_103 n n 0.
+Proof. intros n H; unfold binary_safe_103 in H; tauto. Qed.
+
+Lemma binary_safe_count_step_103 : forall n x bits,
+  binary_safe_103 n ->
+  binary_count_state_z_103 n x bits ->
+  0 < x ->
+  binary_count_state_z_103 n (Z.quot x 2) (bits + 1).
+Proof.
+  intros n x bits Hsafe Hstate Hpos.
+  unfold binary_safe_103 in Hsafe.
+  destruct Hsafe as [_ [_ [_ [_ [Hstep _]]]]].
+  apply Hstep; assumption.
+Qed.
+
+Lemma binary_safe_count_final_103 : forall n bits,
+  binary_safe_103 n ->
+  0 < n ->
+  binary_count_state_z_103 n 0 bits ->
+  bits = binary_length_z_103 n.
+Proof.
+  intros n bits Hsafe Hpos Hstate.
+  unfold binary_safe_103 in Hsafe.
+  destruct Hsafe as [_ [_ [_ [_ [_ [Hfinal _]]]]]].
+  apply Hfinal; assumption.
+Qed.
+
+Lemma binary_safe_length_pos_103 : forall n bits,
+  binary_safe_103 n ->
+  0 < n ->
+  bits = binary_length_z_103 n ->
+  1 <= bits.
+Proof.
+  intros n bits Hsafe Hpos Hbits.
+  unfold binary_safe_103 in Hsafe.
+  destruct Hsafe as [_ [_ [_ [_ [_ [_ [Hlen _]]]]]]].
+  apply Hlen; assumption.
+Qed.
+
+Lemma binary_safe_backfill_initial_103 : forall n bits,
+  binary_safe_103 n ->
+  0 < n ->
+  bits = binary_length_z_103 n ->
+  binary_backfill_state_z_103 n n bits [0].
+Proof.
+  intros n bits Hsafe Hpos Hbits.
+  unfold binary_safe_103 in Hsafe.
+  destruct Hsafe as [_ [_ [_ [_ [_ [_ [_ [Hinit _]]]]]]]].
+  apply Hinit; assumption.
+Qed.
+
+Lemma binary_safe_backfill_step_103 : forall n rem pos suffix,
+  binary_safe_103 n ->
+  binary_backfill_state_z_103 n rem pos suffix ->
+  0 < rem ->
+  0 < pos /\
+  0 <= 48 + Z.rem rem 2 <= 127 /\
+  binary_backfill_state_z_103
+    n (Z.quot rem 2) (pos - 1) ((48 + Z.rem rem 2) :: suffix).
+Proof.
+  intros n rem pos suffix Hsafe Hstate Hpos.
+  unfold binary_safe_103 in Hsafe.
+  destruct Hsafe as [_ [_ [_ [_ [_ [_ [_ [_ [Hstep _]]]]]]]]].
+  apply Hstep; assumption.
+Qed.
+
+Lemma binary_safe_backfill_final_103 : forall n suffix,
+  binary_safe_103 n ->
+  binary_backfill_state_z_103 n 0 0 suffix ->
+  suffix = binary_output_z_103 n ++ [0].
+Proof.
+  intros n suffix Hsafe Hstate.
+  unfold binary_safe_103 in Hsafe.
+  destruct Hsafe as [_ [_ [_ [_ [_ [_ [_ [_ [_ Hfinal]]]]]]]]].
+  apply Hfinal; assumption.
+Qed.
+
+Lemma binary_backfill_zero_pos_103 : forall n pos suffix,
+  binary_backfill_state_z_103 n 0 pos suffix ->
+  pos = 0.
+Proof.
+  intros n pos suffix Hstate.
+  unfold binary_backfill_state_z_103 in Hstate.
+  destruct Hstate as (done & Hnpos & _ & _ & Hbits & Hpos & _).
+  simpl in Hbits. rewrite app_nil_r in Hbits. subst done.
+  unfold binary_length_z_103, binary_output_z_103 in Hpos.
+  destruct n as [|p|p]; try lia; simpl in *.
+  rewrite !Zlength_correct, length_map, length_rev in Hpos.
+  lia.
+Qed.
+
+Lemma binary_safe_zero_output_103 : forall n,
+  binary_safe_103 n ->
+  n = 0 ->
+  binary_output_z_103 n = [48].
+Proof.
+  intros n H ->. unfold binary_safe_103 in H. tauto.
+Qed.
+
+Lemma rounded_avg_safe_use_103 : forall n m,
+  rounded_avg_safe_103 n m ->
+  n <= m ->
+  let avg := Z.quot (n + m) 2 in
+  0 < avg <= INT_MAX /\
+  avg = (n + m) / 2 /\
+  binary_safe_103 avg.
+Proof.
+  intros n m Hsafe Hle. unfold rounded_avg_safe_103 in Hsafe.
+  apply Hsafe; assumption.
+Qed.
+
+Lemma positive_bits_nonempty_103 : forall p,
+  positive_bits_103 p <> [].
+Proof.
+  destruct p; discriminate.
+Qed.
+
+Lemma positive_bits_bound_103 : forall p,
+  list_within_bound 2 (positive_bits_103 p).
+Proof.
+  induction p; simpl; intuition lia.
+Qed.
+
+Lemma positive_bits_value_103 : forall p,
+  list_to_Z 2 (positive_bits_103 p) = Z.pos p.
+Proof.
+  induction p; simpl [positive_bits_103].
+  - rewrite list_to_Z_cons, IHp. rewrite Pos2Z.inj_xI. lia.
+  - rewrite list_to_Z_cons, IHp. rewrite Pos2Z.inj_xO. lia.
+  - rewrite list_to_Z_single. reflexivity.
+Qed.
+
+Lemma positive_bits_last_103 : forall p,
+  last (positive_bits_103 p) 0 = 1.
+Proof.
+  induction p as [p IH | p IH |].
+  - simpl [positive_bits_103].
+    destruct (positive_bits_103 p) eqn:Hbits.
+    + exfalso. apply (positive_bits_nonempty_103 p). assumption.
+    + exact IH.
+  - simpl [positive_bits_103].
+    destruct (positive_bits_103 p) eqn:Hbits.
+    + exfalso. apply (positive_bits_nonempty_103 p). assumption.
+    + exact IH.
+  - reflexivity.
+Qed.
+
+Lemma binary_bits_values_103 : forall n,
+  0 <= n ->
+  Forall (fun b => b = 0 \/ b = 1) (binary_bits_z_103 n).
+Proof.
+  intros n Hn.
+  destruct n as [|p|p]; try lia; simpl.
+  - constructor; [left; reflexivity | constructor].
+  - induction p; simpl; constructor; intuition.
+Qed.
+
+Lemma binary_bits_rel_103 : forall n,
+  0 <= n ->
+  binary_digits (Z.to_nat n) (binary_bits_z_103 n).
+Proof.
+  intros n Hn.
+  destruct n as [|p|p]; try lia.
+  - unfold binary_digits, binary_bits_z_103; simpl.
+    rewrite list_to_Z_single. repeat split; auto.
+  - unfold binary_digits, binary_bits_z_103; simpl.
+    split; [apply positive_bits_bound_103 |].
+    split.
+    + rewrite positive_bits_value_103. symmetry. apply positive_nat_Z.
+    + right. repeat split.
+      * pose proof (Pos2Nat.is_pos p). lia.
+      * apply positive_bits_nonempty_103.
+      * apply positive_bits_last_103.
+Qed.
+
+Lemma string_of_list_z_bit_codes_103 : forall bits,
+  Forall (fun b => b = 0 \/ b = 1) bits ->
+  string_of_list_z_103 (map bit_code_z_103 bits) =
+  string_of_list_ascii (map bit_char bits).
+Proof.
+  intros bits Hbits.
+  induction Hbits as [|b bits Hb Hbits IH]; simpl.
+  - reflexivity.
+  - destruct Hb as [-> | ->]; simpl; rewrite IH; reflexivity.
+Qed.
+
+Lemma binary_output_string_103 : forall n,
+  0 <= n ->
+  string_of_list_z_103 (binary_output_z_103 n) =
+  binary_string_from_digits (binary_bits_z_103 n).
+Proof.
+  intros n Hn.
+  unfold binary_output_z_103, binary_string_from_digits.
+  apply string_of_list_z_bit_codes_103.
+  apply Forall_rev.
+  apply binary_bits_values_103; assumption.
+Qed.
+
+Lemma problem_103_spec_z_neg : forall n m,
+  n > m ->
+  problem_103_spec_z n m [45; 49].
+Proof.
+  intros n m Hgt.
+  unfold problem_103_spec_z, problem_103_spec.
+  left. split; [assumption | reflexivity].
+Qed.
+
+Lemma problem_103_spec_z_binary : forall n m avg,
+  n <= m ->
+  0 <= avg ->
+  avg = (n + m) / 2 ->
+  problem_103_spec_z n m (binary_output_z_103 avg).
+Proof.
+  intros n m avg Hle Havg Hvalue.
+  unfold problem_103_spec_z, problem_103_spec.
+  right.
+  exists (Z.to_nat avg), (binary_bits_z_103 avg).
+  split; [exact Hle |].
+  split.
+  - rewrite Z2Nat.id by lia. exact Hvalue.
+  - split.
+    + apply binary_bits_rel_103; assumption.
+    + apply binary_output_string_103; assumption.
+Qed.
